Kinding.v
@@ -11,6 +11,63 @@ Hint Constructors
      type_equal_core type_equal_cong type_equal_symm type_equal.
 
 (* *************************************************************** *)
+(** * Retraction of valid environments *)
+
+Lemma valid_env_retract : forall E F,
+    valid_env (E & F) -> valid_env E.
+Proof.
+  introv He.
+  induction F using env_ind;
+    autorewrite with rew_env_concat in *; auto.
+  remember (E & F & x ~ v) as G.
+  destruct He.
+  - destruct (empty_concat_inv HeqG) as [_ Hem].
+    apply empty_single_inv in Hem.
+    contradiction.
+  - destruct (eq_push_inv HeqG) as [_ [_ Hem]].
+    rewrite Hem in He.
+    auto.
+  - destruct (eq_push_inv HeqG) as [_ [_ Hem]].
+    rewrite Hem in He.
+    auto.
+Qed.
+
+(* *************************************************************** *)
+(** * Convenient inversions of valid environments *)
+
+Lemma valid_env_kind_inv : forall E X K,
+    valid_env (E & X ~:: K) ->
+    valid_env E /\ X # E /\ valid_kind E K.
+Proof.
+  introv He.
+  remember (E & X ~:: K) as F eqn:Hf.
+  destruct He.
+  - apply empty_push_inv in Hf; contradiction.
+  - destruct (eq_push_inv Hf) as [? [Hk ?]].
+    inversion Hk.
+    subst.
+    auto.
+  - destruct (eq_push_inv Hf) as [_ [Hk _]].
+    discriminate.
+Qed.
+
+Lemma valid_env_type_inv : forall E x M,
+    valid_env (E & x ~: M) ->
+    valid_env E /\ x # E /\ valid_scheme E M.
+Proof.
+  introv He.
+  remember (E & x ~: M) as F eqn:Hf.
+  destruct He.
+  - apply empty_push_inv in Hf; contradiction.
+  - destruct (eq_push_inv Hf) as [_ [Hm _]].
+    discriminate.
+  - destruct (eq_push_inv Hf) as [? [Hm ?]].
+    inversion Hm.
+    subst.
+    auto.
+Qed.
+
+(* *************************************************************** *)
 (** Weakening *)
 
 Lemma combined_kinding_weakening :
@@ -107,6 +164,16 @@ Proof.
   intuition assumption.
 Qed.
 
+Lemma valid_kind_weakening_l : forall E F K,
+    valid_kind E K ->
+    valid_env (E & F) ->
+    valid_kind (E & F) K.
+Proof.
+  introv Hv He.
+  rewrite <- concat_empty_r with (E := E & F).
+  apply valid_kind_weakening; rewrite concat_empty_r; assumption.
+Qed.
+
 Lemma kinding_weakening : forall E F G T K,
    kinding (E & G) T K -> 
    valid_env (E & F & G) ->
@@ -123,6 +190,16 @@ Proof.
   generalize dependent EG.
   pose combined_kinding_weakening.
   intuition assumption.
+Qed.
+
+Lemma kinding_weakening_l : forall E F T K,
+   kinding E T K -> 
+   valid_env (E & F) ->
+   kinding (E & F) T K.
+Proof.
+  introv Hv He.
+  rewrite <- concat_empty_r with (E := E & F).
+  apply kinding_weakening; rewrite concat_empty_r; assumption.
 Qed.
 
 Lemma valid_scheme_vars_weakening : forall E F G M Xs,
@@ -146,7 +223,19 @@ Proof.
   pose combined_kinding_weakening.
   intuition assumption.
 Qed.
-    
+
+Lemma valid_scheme_vars_weakening_l : forall E F M Xs,
+    fresh (dom F) (sch_arity M) Xs ->
+    valid_scheme_vars E M Xs ->
+    valid_env (E & F) ->
+    valid_scheme_vars (E & F) M Xs.
+Proof.
+  introv Hv He.
+  rewrite <- concat_empty_r with (E := E & F).
+  apply valid_scheme_vars_weakening;
+    rewrite? concat_empty_r; assumption.
+Qed.
+
 Lemma valid_scheme_weakening : forall E F G M,
     valid_scheme (E & G) M ->
     valid_env (E & F & G) ->
@@ -163,6 +252,16 @@ Proof.
   pose combined_kinding_weakening.
   intuition assumption.
 Qed.  
+
+Lemma valid_scheme_weakening_l : forall E F M,
+    valid_scheme E M ->
+    valid_env (E & F) ->
+    valid_scheme (E & F) M.
+Proof.
+  introv Hv He.
+  rewrite <- concat_empty_r with (E := E & F).
+  apply valid_scheme_weakening; rewrite concat_empty_r; assumption.
+Qed.
 
 Lemma type_equal_core_weakening : forall E F G T1 T2 K,
    type_equal_core (E & G) T1 T2 K -> 
@@ -181,6 +280,16 @@ Proof.
   generalize dependent EG.
   pose combined_kinding_weakening.
   intuition assumption.
+Qed.
+
+Lemma type_equal_core_weakening_l : forall E F T1 T2 K,
+   type_equal_core E T1 T2 K -> 
+   valid_env (E & F) ->
+   type_equal_core (E & F) T1 T2 K.
+Proof.
+  introv Hv He.
+  rewrite <- concat_empty_r with (E := E & F).
+  apply type_equal_core_weakening; rewrite concat_empty_r; assumption.
 Qed.
 
 Lemma type_equal_cong_weakening : forall E F G T1 T2 K,
@@ -202,6 +311,16 @@ Proof.
   intuition assumption.
 Qed.
 
+Lemma type_equal_cong_weakening_l : forall E F T1 T2 K,
+   type_equal_cong E T1 T2 K -> 
+   valid_env (E & F) ->
+   type_equal_cong (E & F) T1 T2 K.
+Proof.
+  introv Hv He.
+  rewrite <- concat_empty_r with (E := E & F).
+  apply type_equal_cong_weakening; rewrite concat_empty_r; assumption.
+Qed.
+
 Lemma type_equal_symm_weakening : forall E F G T1 T2 K,
    type_equal_symm (E & G) T1 T2 K -> 
    valid_env (E & F & G) ->
@@ -219,6 +338,16 @@ Proof.
   generalize dependent EG.
   pose combined_kinding_weakening.
   intuition assumption.
+Qed.
+
+Lemma type_equal_symm_weakening_l : forall E F T1 T2 K,
+   type_equal_symm E T1 T2 K -> 
+   valid_env (E & F) ->
+   type_equal_symm (E & F) T1 T2 K.
+Proof.
+  introv Hv He.
+  rewrite <- concat_empty_r with (E := E & F).
+  apply type_equal_symm_weakening; rewrite concat_empty_r; assumption.
 Qed.
 
 Lemma type_equal_weakening : forall E F G T1 T2 K,
@@ -240,6 +369,16 @@ Proof.
   intuition assumption.
 Qed.
 
+Lemma type_equal_weakening_l : forall E F T1 T2 K,
+   type_equal E T1 T2 K -> 
+   valid_env (E & F) ->
+   type_equal (E & F) T1 T2 K.
+Proof.
+  introv Hv He.
+  rewrite <- concat_empty_r with (E := E & F).
+  apply type_equal_weakening; rewrite concat_empty_r; assumption.
+Qed.
+
 Lemma subtype_weakening : forall E F G T1 T2 cs,
     subtype (E & G) T1 T2 cs ->
     valid_env (E & F & G) ->
@@ -259,6 +398,16 @@ Proof.
   intuition assumption.
 Qed.
 
+Lemma subtype_weakening_l : forall E F T1 T2 cs,
+    subtype E T1 T2 cs ->
+    valid_env (E & F) ->
+    subtype (E & F) T1 T2 cs.
+Proof.
+  introv Hv He.
+  rewrite <- concat_empty_r with (E := E & F).
+  apply subtype_weakening; rewrite concat_empty_r; assumption.
+Qed.
+
 Lemma valid_instance_weakening : forall E F G Ts M,
   valid_instance (E & G) Ts M ->
   valid_env (E & F & G) ->
@@ -266,60 +415,17 @@ Lemma valid_instance_weakening : forall E F G Ts M,
 Proof.
   introv Hk He.
   remember (E & G) as EG.
-  induction Hk; subst.
-  - apply valid_instance_empty.
-  - auto using kinding_weakening.
+  induction Hk; subst; auto using kinding_weakening.
 Qed.
 
-Lemma valid_env_retract : forall E F,
-    valid_env (E & F) -> valid_env E.
+Lemma valid_instance_weakening_l : forall E F Ts M,
+  valid_instance E Ts M ->
+  valid_env (E & F) ->
+  valid_instance (E & F) Ts M.
 Proof.
-  introv He.
-  induction F using env_ind;
-    autorewrite with rew_env_concat in *; auto.
-  remember (E & F & x ~ v) as G.
-  destruct He.
-  - destruct (empty_concat_inv HeqG) as [_ Hem].
-    apply empty_single_inv in Hem.
-    contradiction.
-  - destruct (eq_push_inv HeqG) as [_ [_ Hem]].
-    rewrite Hem in He.
-    auto.
-  - destruct (eq_push_inv HeqG) as [_ [_ Hem]].
-    rewrite Hem in He.
-    auto.
-Qed.
-
-Lemma valid_env_kind_inv : forall E X K,
-    valid_env (E & X ~:: K) ->
-    valid_kind E K /\ X # E.
-Proof.
-  introv He.
-  remember (E & X ~:: K) as F eqn:Hf.
-  destruct He.
-  - apply empty_push_inv in Hf; contradiction.
-  - destruct (eq_push_inv Hf) as [? [Hk ?]].
-    inversion Hk.
-    subst.
-    auto.
-  - destruct (eq_push_inv Hf) as [_ [Hk _]].
-    discriminate.
-Qed.
-
-Lemma valid_env_type_inv : forall E x M,
-    valid_env (E & x ~: M) ->
-    valid_scheme E M /\ x # E.
-Proof.
-  introv He.
-  remember (E & x ~: M) as F eqn:Hf.
-  destruct He.
-  - apply empty_push_inv in Hf; contradiction.
-  - destruct (eq_push_inv Hf) as [_ [Hm _]].
-    discriminate.
-  - destruct (eq_push_inv Hf) as [? [Hm ?]].
-    inversion Hm.
-    subst.
-    auto.
+  introv Hv He.
+  rewrite <- concat_empty_r with (E := E & F).
+  apply valid_instance_weakening; rewrite concat_empty_r; assumption.
 Qed.
 
 Lemma valid_env_kind_weakening : forall E F G X K,
@@ -331,8 +437,19 @@ Proof.
   introv Hin He1 He2.
   assert (environment (E & F & G))
     by auto with valid_env_regular.
-  destruct (valid_env_kind_inv He1).
+  destruct (valid_env_kind_inv He1) as [_ [? ?]].
   auto using valid_kind_weakening.
+Qed.
+
+Lemma valid_env_kind_weakening_l : forall E F X K,
+    X # F ->
+    valid_env (E & X ~:: K) ->
+    valid_env (E & F) ->
+    valid_env (E & F & X ~:: K).
+Proof.
+  introv Hv He.
+  rewrite <- concat_empty_r with (E := E & F).
+  apply valid_env_kind_weakening; rewrite? concat_empty_r; assumption.
 Qed.
 
 Lemma valid_env_type_weakening : forall E F G x M,
@@ -344,8 +461,19 @@ Proof.
   introv Hin He1 He2.
   assert (environment (E & F & G))
     by auto with valid_env_regular.
-  destruct (valid_env_type_inv He1).
+  destruct (valid_env_type_inv He1) as [_ [? ?]].
   auto using valid_scheme_weakening.
+Qed.
+
+Lemma valid_env_type_weakening_l : forall E F x M,
+    x # F ->
+    valid_env (E & x ~: M) ->
+    valid_env (E & F) ->
+    valid_env (E & F & x ~: M).
+Proof.
+  introv Hv He.
+  rewrite <- concat_empty_r with (E := E & F).
+  apply valid_env_type_weakening; rewrite? concat_empty_r; assumption.
 Qed.
 
 Lemma valid_env_kinds_weakening : forall E F G Xs M,
@@ -377,6 +505,21 @@ Proof.
     apply valid_env_kind_weakening;
       eauto using valid_env_retract.
 Qed.
+
+Lemma valid_env_kinds_weakening_l : forall E F Xs M,
+    fresh (dom F) (sch_arity M) Xs ->
+    valid_env (E & Xs ~::* M) ->
+    valid_env (E & F) ->
+    valid_env (E & F & Xs ~::* M).
+Proof.
+  introv Hv He.
+  rewrite <- concat_empty_r with (E := E & F).
+  apply valid_env_kinds_weakening;
+    rewrite? concat_empty_r; assumption.
+Qed.
+
+(* *************************************************************** *)
+(** * Valid bindings *)
 
 Lemma valid_scheme_from_env : forall E x M,
     valid_env E ->
@@ -417,475 +560,3106 @@ Proof.
 Qed.
 
 (* *************************************************************** *)
+(** Judegments are closed *)
+
+Lemma combined_kinding_closed :
+     (forall E K,
+      valid_kind_regular E K ->
+      (forall X,
+          X # E ->
+          X \notin (knd_fv K)))
+  /\ (forall E T K,
+      kinding_regular E T K ->
+         (forall X,
+          X # E ->
+          X \notin (typ_fv T))
+      /\ (forall X,
+          X # E ->
+          X \notin (knd_fv K)))
+  /\ (forall E M Xs,
+      valid_scheme_vars_regular E M Xs ->
+      (forall X,
+          fresh \{X} (sch_arity M) Xs ->
+          X # E ->
+          X \notin (sch_fv M)))
+  /\ (forall E M,
+      valid_scheme_regular E M ->
+      (forall X,
+          X # E ->
+          X \notin (sch_fv M)))
+  /\ (forall E,
+      valid_env_regular E ->
+      (forall X Y K,
+          X # E ->
+          binds Y (bind_knd K) E ->
+          X \notin (knd_fv K)))
+  /\ (forall E T1 T2 K,
+      type_equal_core_regular E T1 T2 K ->
+         (forall X,
+          X # E ->
+          X \notin (typ_fv T1))
+      /\ (forall X,
+          X # E ->
+          X \notin (typ_fv T2))
+      /\ (forall X,
+          X # E ->
+          X \notin (knd_fv K)))
+  /\ (forall E T1 T2 K,
+      type_equal_cong_regular E T1 T2 K ->
+         (forall X,
+          X # E ->
+          X \notin (typ_fv T1))
+      /\ (forall X,
+          X # E ->
+          X \notin (typ_fv T2))
+      /\ (forall X,
+          X # E ->
+          X \notin (knd_fv K)))
+  /\ (forall E T1 T2 K,
+      type_equal_symm_regular E T1 T2 K ->
+         (forall X,
+          X # E ->
+          X \notin (typ_fv T1))
+      /\ (forall X,
+          X # E ->
+          X \notin (typ_fv T2))
+      /\ (forall X,
+          X # E ->
+          X \notin (knd_fv K)))
+  /\ (forall E T1 T2 K,
+      type_equal_regular E T1 T2 K ->
+         (forall X,
+          X # E ->
+          X \notin (typ_fv T1))
+      /\ (forall X,
+          X # E ->
+          X \notin (typ_fv T2))
+      /\ (forall X,
+          X # E ->
+          X \notin (knd_fv K)))
+  /\ (forall E T1 T2 cs,
+      subtype_regular E T1 T2 cs ->
+         (forall X,
+          X # E ->
+          X \notin (typ_fv T1))
+      /\ (forall X,
+          X # E ->
+          X \notin (typ_fv T2))).
+Proof.      
+  apply combined_kinding_regular_mutind; jauto_set; intros; subst;
+    simpl; auto.
+  - apply notin_singleton_l.
+    intro; subst.
+    eauto using get_some_inv, binds_get.
+  - eauto.
+  - autorewrite with rew_sch_arity in *.
+    eauto using sch_open_var_fv.
+  - pick_freshes_gen (L \u \{X}) (sch_arity M) Xs.
+    eauto.
+  - exfalso.
+    eapply binds_empty_inv.
+    eassumption.
+  - assert (binds Y (bind_knd K0) (E & X ~:: K)) as Hb by assumption.
+    destruct (binds_push_inv Hb) as [[Heq1 Heq2]|[Hneq Hb2]].
+    + inversion Heq2; auto.
+    + eauto.
+  - assert (binds Y (bind_knd K) (E & x ~: M)) as Hb by assumption.
+    destruct (binds_push_inv Hb) as [[Heq1 Heq2]|[Hneq Hb2]].
+    + discriminate.
+    + eauto.
+  - assert (X \notin (typ_fv T1) \u (typ_fv T2))
+      by (simpl in *; auto).
+    auto.
+Qed.
+
+Lemma valid_kind_closed : forall E K X,
+    valid_kind E K ->
+    X # E ->
+    X \notin (knd_fv K).
+Proof.
+  introv Hk Hn.
+  apply regular_valid_kind in Hk.
+  pose combined_kinding_closed.
+  intuition eauto.
+Qed.
+
+Lemma kinding_closed : forall E T K X,
+    kinding E T K ->
+    X # E ->
+    X \notin ((typ_fv T) \u (knd_fv K)).
+Proof.
+  introv Hk Hn.
+  apply regular_kinding in Hk.
+  pose combined_kinding_closed.
+  jauto_set.
+  assert
+    ((forall X : var, X # E -> X \notin typ_fv T)
+  /\ (forall X : var, X # E -> X \notin knd_fv K)) as Hc by auto.
+  intuition auto.
+Qed.
+
+Lemma valid_scheme_vars_closed : forall E M Xs X,
+    valid_scheme_vars E M Xs ->
+    fresh \{X} (sch_arity M) Xs ->
+    X # E ->
+    X \notin (sch_fv M).
+Proof.
+  introv Hs Hn.
+  apply regular_valid_scheme_vars in Hs.
+  pose combined_kinding_closed.
+  intuition eauto.
+Qed.
+
+Lemma valid_scheme_closed : forall E M X,
+    valid_scheme E M ->
+    X # E ->
+    X \notin (sch_fv M).
+Proof.
+  introv Hs Hn.
+  apply regular_valid_scheme in Hs.
+  pose combined_kinding_closed.
+  intuition eauto.
+Qed.
+
+Lemma valid_env_binds_knd_closed : forall E X Y K,
+    valid_env E ->
+    X # E ->
+    binds Y (bind_knd K) E ->
+    X \notin (knd_fv K).
+Proof.
+  introv He Hn.
+  apply regular_valid_env in He.
+  pose combined_kinding_closed.
+  intuition eauto.
+Qed.
+
+Lemma valid_env_knd_closed : forall E X K,
+    valid_env (E & X ~:: K) ->
+    X # E ->
+    X \notin knd_fv K.
+Proof.
+  introv He Hn.
+  remember (E & X ~:: K) as EX.
+  induction He; intros; subst.
+  - exfalso. eapply empty_push_inv. eassumption.
+  - destruct (eq_push_inv HeqEX) as [? [HeqK ?]].
+    inversion HeqK; subst.
+    eauto using valid_kind_closed.
+  - destruct (eq_push_inv HeqEX) as [? [HeqK ?]].
+    discriminate.
+Qed.
+
+Lemma type_equal_core_closed : forall E T1 T2 K X,
+    type_equal_core E T1 T2 K ->
+    X # E ->
+    X \notin ((typ_fv T1) \u (typ_fv T2) \u (knd_fv K)).
+Proof.
+  introv Hte Hn.
+  apply regular_type_equal_core in Hte.
+  pose combined_kinding_closed.
+  jauto_set.
+  assert
+    ((forall X : var, X # E -> X \notin typ_fv T1)
+  /\ (forall X : var, X # E -> X \notin typ_fv T2)
+  /\ (forall X : var, X # E -> X \notin knd_fv K)) as Hc by auto.
+  intuition auto.
+Qed.
+
+Lemma type_equal_cong_closed : forall E T1 T2 K X,
+    type_equal_cong E T1 T2 K ->
+    X # E ->
+    X \notin ((typ_fv T1) \u (typ_fv T2) \u (knd_fv K)).
+Proof.
+  introv Hte Hn.
+  apply regular_type_equal_cong in Hte.
+  pose combined_kinding_closed.
+  jauto_set.
+  assert
+    ((forall X : var, X # E -> X \notin typ_fv T1)
+  /\ (forall X : var, X # E -> X \notin typ_fv T2)
+  /\ (forall X : var, X # E -> X \notin knd_fv K)) as Hc by auto.
+  intuition auto.
+Qed.
+
+Lemma type_equal_symm_closed : forall E T1 T2 K X,
+    type_equal_symm E T1 T2 K ->
+    X # E ->
+    X \notin ((typ_fv T1) \u (typ_fv T2) \u (knd_fv K)).
+Proof.
+  introv Hte Hn.
+  apply regular_type_equal_symm in Hte.
+  pose combined_kinding_closed.
+  jauto_set.
+  assert
+    ((forall X : var, X # E -> X \notin typ_fv T1)
+  /\ (forall X : var, X # E -> X \notin typ_fv T2)
+  /\ (forall X : var, X # E -> X \notin knd_fv K)) as Hc by auto.
+  intuition auto.
+Qed.
+
+Lemma type_equal_closed : forall E T1 T2 K X,
+    type_equal E T1 T2 K ->
+    X # E ->
+    X \notin ((typ_fv T1) \u (typ_fv T2) \u (knd_fv K)).
+Proof.
+  introv Hte Hn.
+  apply regular_type_equal in Hte.
+  pose combined_kinding_closed.
+  jauto_set.
+  assert
+    ((forall X : var, X # E -> X \notin typ_fv T1)
+  /\ (forall X : var, X # E -> X \notin typ_fv T2)
+  /\ (forall X : var, X # E -> X \notin knd_fv K)) as Hc by auto.
+  intuition auto.
+Qed.
+
+Lemma subtype_closed : forall E T1 T2 cs X,
+    subtype E T1 T2 cs ->
+    X # E ->
+    X \notin ((typ_fv T1) \u (typ_fv T2)).
+Proof.
+  introv Hs Hn.
+  apply regular_subtype in Hs.
+  pose combined_kinding_closed.
+  jauto_set.
+  assert
+    ((forall X : var, X # E -> X \notin typ_fv T1)
+  /\ (forall X : var, X # E -> X \notin typ_fv T2)) as Hc by eauto.
+  intuition auto.
+Qed.
+
+Lemma valid_instance_closed : forall E Ts M X,
+  valid_instance E Ts M ->
+  X # E ->
+  X \notin ((typ_fv_list Ts) \u (sch_fv M)).
+Proof.
+  introv Hi Hn.
+  induction Hi; simpl.
+  - assert (kinding E T knd_type) as Hk by assumption.
+    apply kinding_closed with (X := X) in Hk; auto.
+  - assert (kinding E T K) as Hk by assumption.
+    apply kinding_closed with (X := X) in Hk; auto.
+    assert (X \notin typ_fv_list Ts \u sch_fv (sch_open M T)) as Hn2
+      by auto.
+    eauto using sch_open_fv.
+Qed.
+
+(* *************************************************************** *)
 (** Preserved by type substitution *)
 
-Lemma kinding_core_typ_subst : forall E X T S K J,
-  kinding_core (E & X ~:: J) T K -> 
-  kinding E S J -> 
-  kinding E (typ_subst X S T) K.
+Lemma combined_kinding_typ_subst :
+     (forall EXF K,
+      valid_kind_regular EXF K ->
+      (forall E F X J S,
+          EXF = E & X ~:: J & F ->
+          kinding E S J ->
+          valid_kind (E & env_subst X S F) (knd_subst X S K)))
+  /\ (forall EXF T K,
+      kinding_regular EXF T K ->
+      (forall E F X J S,
+          EXF = E & X ~:: J & F ->
+          kinding E S J ->
+          kinding (E & env_subst X S F)
+            (typ_subst X S T) (knd_subst X S K)))
+  /\ (forall EXF M Xs,
+      valid_scheme_vars_regular EXF M Xs ->
+      (forall E F X J S,
+          fresh \{X} (sch_arity M) Xs ->
+          EXF = E & X ~:: J & F ->
+          kinding E S J ->
+          valid_scheme_vars (E & env_subst X S F)
+            (sch_subst X S M) Xs))
+  /\ (forall EXF M,
+      valid_scheme_regular EXF M ->
+      (forall E F X J S,
+          EXF = E & X ~:: J & F ->
+          kinding E S J ->
+          valid_scheme (E & env_subst X S F) (sch_subst X S M)))
+  /\ (forall EXF,
+      valid_env_regular EXF ->
+      (forall E F X J S,
+          EXF = E & X ~:: J & F ->
+          kinding E S J ->
+          valid_env (E & env_subst X S F)))
+  /\ (forall EXF T1 T2 K,
+      type_equal_core_regular EXF T1 T2 K ->
+      (forall E F X J S,
+          EXF = E & X ~:: J & F ->
+          kinding E S J ->
+          type_equal_core (E & env_subst X S F)
+            (typ_subst X S T1) (typ_subst X S T2) (knd_subst X S K)))
+  /\ (forall EXF T1 T2 K,
+      type_equal_cong_regular EXF T1 T2 K ->
+      (forall E F X J S,
+          EXF = E & X ~:: J & F ->
+          kinding E S J ->
+          type_equal_cong (E & env_subst X S F)
+            (typ_subst X S T1) (typ_subst X S T2) (knd_subst X S K)))
+  /\ (forall EXF T1 T2 K,
+      type_equal_symm_regular EXF T1 T2 K ->
+      (forall E F X J S,
+          EXF = E & X ~:: J & F ->
+          kinding E S J ->
+          type_equal_symm (E & env_subst X S F)
+            (typ_subst X S T1) (typ_subst X S T2) (knd_subst X S K)))
+  /\ (forall EXF T1 T2 K,
+      type_equal_regular EXF T1 T2 K ->
+      (forall E F X J S,
+          EXF = E & X ~:: J & F ->
+          kinding E S J ->
+          type_equal (E & env_subst X S F)
+            (typ_subst X S T1) (typ_subst X S T2) (knd_subst X S K)))
+  /\ (forall EXF T1 T2 cs,
+      subtype_regular EXF T1 T2 cs ->
+      (forall E F X J S,
+          EXF = E & X ~:: J & F ->
+          kinding E S J ->
+          subtype (E & env_subst X S F)
+            (typ_subst X S T1) (typ_subst X S T2) cs)).
 Proof.
-  introv Hkc Hk.
-  apply regular_kinding_core in Hkc.
-  remember (E & X ~:: J) as F.
-  induction Hkc; subst; simpl.
+  apply combined_kinding_regular_mutind; intros; subst; simpl;
+    econstr eauto.
   - case_var.
-    + assert (binds X (bind_knd K) (E & X ~:: J)) as Hb
-        by assumption.
-      apply binds_push_eq_inv in Hb.
-      inversion Hb; subst.
-      assumption.
-    + assert (binds X0 (bind_knd K) (E & X ~:: J)) as Hb
-        by assumption.
-      apply binds_push_neq_inv in Hb; try assumption.
-      assert (kinding_core E (typ_fvar X0) K)
+    + assert (bind_knd K = bind_knd J) as Hbnd
+        by eauto using binds_middle_eq_inv, ok_from_environment.
+      inversion Hbnd; subst.
+      rewrite knd_subst_fresh; eauto using kinding_weakening_l.
+      assert (environment (E0 & X0 ~:: J)) as He
         by eauto using environment_retract.
-      
+      destruct (environment_knd_inv He).
+      eauto using valid_env_knd_closed, valid_env_retract.
+    + { assert (binds X (bind_knd K) (E0 & X0 ~:: J & F)) as Hb
+          by assumption.
+        destruct (binds_middle_inv Hb)
+          as [Hbf | [[Hn [Heq1 Heq2]] | [Hn [Hneq Hbe]]]].
+        - apply env_subst_binds with (Z := X0) (U := S) in Hbf.
+          simpl in Hbf.
+          apply binds_concat_right with (E1 := E0) in Hbf.
+          eauto.
+        - contradiction.
+        - assert (environment (E0 & X0 ~:: J)) as He
+            by eauto using environment_retract.
+          destruct (environment_knd_inv He).
+          assert (valid_env E0) by eauto using valid_env_retract.
+          rewrite knd_subst_fresh; eauto using kinding_weakening_l.
+          apply valid_env_binds_knd_closed
+            with (E := E0) (Y := X); auto. }
+  - apply kinding_variant
+      with (T1 := typ_subst X S T1) (T2 := typ_subst X S T2).
+    eauto.
+  - apply kinding_range_subsumption
+      with (T1 := typ_subst X S T1) (T2 := typ_subst X S T2); eauto.
+  - apply valid_scheme_vars_bind; eauto.
+    rewrite <- concat_assoc.
+    rewrite <- env_subst_knd.
+    rewrite sch_subst_open_var; auto with kinding_regular.
+    assert (fresh \{X0} (sch_arity (sch_bind K M)) (X :: Xs)) as Hf
+      by assumption.
+    destruct Hf as [? Hf].
+    rewrite <- sch_open_var_arity with (X := X) in Hf.
+    eauto using concat_assoc.
+  - apply valid_scheme_c with (L := L \u \{X}).
+    autorewrite with rew_sch_arity.
+    eauto.
+  - exfalso. eapply empty_middle_inv. eassumption.
+  - assert (E & X ~:: K = E0 & X0 ~:: J & F) as Heq
+      by assumption.
+    destruct F using env_ind.
+    + rewrite concat_empty_r in Heq.
+      destruct (eq_push_inv Heq) as [? [Heqb ?]].
+      inversion Heqb; subst.
+      autorewrite with rew_env_subst rew_env_concat.
+      auto.
+    + rewrite concat_assoc in Heq.
+      destruct (eq_push_inv Heq) as [? [? ?]]; subst.
+      autorewrite with rew_env_subst rew_env_concat.
+      simpl.
+      apply valid_env_kind; autorewrite with rew_env_dom; eauto.
+  - assert (E & x ~: M = E0 & X ~:: J & F) as Heq
+      by assumption.
+    destruct F using env_ind.
+    + rewrite concat_empty_r in Heq.
+      destruct (eq_push_inv Heq) as [? [Heqb ?]].
+      discriminate.
+    + rewrite concat_assoc in Heq.
+      destruct (eq_push_inv Heq) as [? [? ?]]; subst.
+      autorewrite with rew_env_subst rew_env_concat.
+      simpl.
+      apply valid_env_type; autorewrite with rew_env_dom; eauto.
+  - apply type_equal_core_or_associative
+      with (cs1 := cs1) (cs2 := cs2) (cs3 := cs3); eauto.
+  - apply type_equal_cong_range_subsumption
+      with (T3 := typ_subst X S T3) (T4 := typ_subst X S T4); eauto.
+Qed.
+
+Lemma valid_kind_typ_subst : forall E F X J S K,
+    valid_kind (E & X ~:: J & F) K ->
+    kinding E S J ->
+    valid_kind (E & env_subst X S F) (knd_subst X S K).
+Proof.
+  introv Hv Hk.
+  apply regular_valid_kind in Hv.
+  pose combined_kinding_typ_subst.
+  intuition eauto.
+Qed.
+
+Lemma valid_kind_typ_subst_l : forall E X J S K,
+    valid_kind (E & X ~:: J) K ->
+    kinding E S J ->
+    valid_kind E (knd_subst X S K).
+Proof.
+  introv Hv Hk.
+  rewrite <- concat_empty_r with (E := E & X ~:: J) in Hv.
+  rewrite <- concat_empty_r with (E := E).
+  rewrite <- env_subst_empty with (X := X) (U := S).
+  eauto using valid_kind_typ_subst.
+Qed.
+
+Lemma kinding_typ_subst : forall E F X J S T K,
+    kinding (E & X ~:: J & F) T K ->
+    kinding E S J ->
+    kinding (E & env_subst X S F)
+      (typ_subst X S T) (knd_subst X S K).
+Proof.
+  introv Hk1 Hk2.
+  apply regular_kinding in Hk1.
+  pose combined_kinding_typ_subst.
+  intuition eauto.
+Qed.
+
+Lemma kinding_typ_subst_l : forall E X J S T K,
+    kinding (E & X ~:: J) T K ->
+    kinding E S J ->
+    kinding E (typ_subst X S T) (knd_subst X S K).
+Proof.
+  introv Hk1 Hk2.
+  rewrite <- concat_empty_r with (E := E & X ~:: J) in Hk1.
+  rewrite <- concat_empty_r with (E := E).
+  rewrite <- env_subst_empty with (X := X) (U := S).
+  eauto using kinding_typ_subst.
+Qed.
+
+Lemma valid_scheme_vars_typ_subst : forall E F X J S M Xs,
+    valid_scheme_vars (E & X ~:: J & F) M Xs ->
+    fresh \{X} (sch_arity M) Xs ->
+    kinding E S J ->
+    valid_scheme_vars (E & env_subst X S F) (sch_subst X S M) Xs.
+Proof.
+  introv Hv Hf Hk.
+  apply regular_valid_scheme_vars in Hv.
+  pose combined_kinding_typ_subst.
+  intuition eauto.
+Qed.
+
+Lemma valid_scheme_vars_typ_subst_l : forall E X J S M Xs,
+    valid_scheme_vars (E & X ~:: J) M Xs ->
+    fresh \{X} (sch_arity M) Xs ->
+    kinding E S J ->
+    valid_scheme_vars E (sch_subst X S M) Xs.
+Proof.
+  introv Hv Hf Hk.
+  rewrite <- concat_empty_r with (E := E & X ~:: J) in Hv.
+  rewrite <- concat_empty_r with (E := E).
+  rewrite <- env_subst_empty with (X := X) (U := S).
+  eauto using valid_scheme_vars_typ_subst.
+Qed.
+
+Lemma valid_scheme_typ_subst : forall E F X J S M,
+    valid_scheme (E & X ~:: J & F) M ->
+    kinding E S J ->
+    valid_scheme (E & env_subst X S F) (sch_subst X S M).
+Proof.
+  introv Hv Hk.
+  apply regular_valid_scheme in Hv.
+  pose combined_kinding_typ_subst.
+  intuition eauto.
+Qed.
+
+Lemma valid_scheme_typ_subst_l : forall E X J S M,
+    valid_scheme (E & X ~:: J) M ->
+    kinding E S J ->
+    valid_scheme E (sch_subst X S M).
+Proof.
+  introv Hv Hk.
+  rewrite <- concat_empty_r with (E := E & X ~:: J) in Hv.
+  rewrite <- concat_empty_r with (E := E).
+  rewrite <- env_subst_empty with (X := X) (U := S).
+  eauto using valid_scheme_typ_subst.
+Qed.
+
+Lemma valid_env_typ_subst: forall E F X J S,
+    valid_env (E & X ~:: J & F) ->
+    kinding E S J ->
+    valid_env (E & env_subst X S F).
+Proof.
+  introv Hv Hk.
+  apply regular_valid_env in Hv.
+  pose combined_kinding_typ_subst.
+  intuition eauto.
+Qed.
+
+Lemma type_equal_core_typ_subst : forall E F X J S T1 T2 K,
+    type_equal_core (E & X ~:: J & F) T1 T2 K ->
+    kinding E S J ->
+    type_equal_core (E & env_subst X S F)
+      (typ_subst X S T1) (typ_subst X S T2) (knd_subst X S K).
+Proof.
+  introv Hte Hk.
+  apply regular_type_equal_core in Hte.
+  pose combined_kinding_typ_subst.
+  intuition eauto.
+Qed.
+
+Lemma type_equal_core_typ_subst_l : forall E X J S T1 T2 K,
+    type_equal_core (E & X ~:: J) T1 T2 K ->
+    kinding E S J ->
+    type_equal_core E
+      (typ_subst X S T1) (typ_subst X S T2) (knd_subst X S K).
+Proof.
+  introv Hte Hk.
+  rewrite <- concat_empty_r with (E := E & X ~:: J) in Hte.
+  rewrite <- concat_empty_r with (E := E).
+  rewrite <- env_subst_empty with (X := X) (U := S).
+  eauto using type_equal_core_typ_subst.
+Qed.
+
+Lemma type_equal_cong_typ_subst : forall E F X J S T1 T2 K,
+    type_equal_cong (E & X ~:: J & F) T1 T2 K ->
+    kinding E S J ->
+    type_equal_cong (E & env_subst X S F)
+      (typ_subst X S T1) (typ_subst X S T2) (knd_subst X S K).
+Proof.
+  introv Hte Hk.
+  apply regular_type_equal_cong in Hte.
+  pose combined_kinding_typ_subst.
+  intuition eauto.
+Qed.
+
+Lemma type_equal_cong_typ_subst_l : forall E X J S T1 T2 K,
+    type_equal_cong (E & X ~:: J) T1 T2 K ->
+    kinding E S J ->
+    type_equal_cong E
+      (typ_subst X S T1) (typ_subst X S T2) (knd_subst X S K).
+Proof.
+  introv Hte Hk.
+  rewrite <- concat_empty_r with (E := E & X ~:: J) in Hte.
+  rewrite <- concat_empty_r with (E := E).
+  rewrite <- env_subst_empty with (X := X) (U := S).
+  eauto using type_equal_cong_typ_subst.
+Qed.
+
+Lemma type_equal_symm_typ_subst : forall E F X J S T1 T2 K,
+    type_equal_symm (E & X ~:: J & F) T1 T2 K ->
+    kinding E S J ->
+    type_equal_symm (E & env_subst X S F)
+      (typ_subst X S T1) (typ_subst X S T2) (knd_subst X S K).
+Proof.
+  introv Hte Hk.
+  apply regular_type_equal_symm in Hte.
+  pose combined_kinding_typ_subst.
+  intuition eauto.
+Qed.
+
+Lemma type_equal_symm_typ_subst_l : forall E X J S T1 T2 K,
+    type_equal_symm (E & X ~:: J) T1 T2 K ->
+    kinding E S J ->
+    type_equal_symm E
+      (typ_subst X S T1) (typ_subst X S T2) (knd_subst X S K).
+Proof.
+  introv Hte Hk.
+  rewrite <- concat_empty_r with (E := E & X ~:: J) in Hte.
+  rewrite <- concat_empty_r with (E := E).
+  rewrite <- env_subst_empty with (X := X) (U := S).
+  eauto using type_equal_symm_typ_subst.
+Qed.
+
+Lemma type_equal_typ_subst : forall E F X J S T1 T2 K,
+    type_equal (E & X ~:: J & F) T1 T2 K ->
+    kinding E S J ->
+    type_equal (E & env_subst X S F)
+      (typ_subst X S T1) (typ_subst X S T2) (knd_subst X S K).
+Proof.
+  introv Hte Hk.
+  apply regular_type_equal in Hte.
+  pose combined_kinding_typ_subst.
+  intuition eauto.
+Qed.
+
+Lemma type_equal_typ_subst_l : forall E X J S T1 T2 K,
+    type_equal (E & X ~:: J) T1 T2 K ->
+    kinding E S J ->
+    type_equal E
+      (typ_subst X S T1) (typ_subst X S T2) (knd_subst X S K).
+Proof.
+  introv Hte Hk.
+  rewrite <- concat_empty_r with (E := E & X ~:: J) in Hte.
+  rewrite <- concat_empty_r with (E := E).
+  rewrite <- env_subst_empty with (X := X) (U := S).
+  eauto using type_equal_typ_subst.
+Qed.
+
+Lemma subtype_typ_subst : forall E F X J S T1 T2 cs,
+    subtype (E & X ~:: J & F) T1 T2 cs ->
+    kinding E S J ->
+    subtype (E & env_subst X S F)
+      (typ_subst X S T1) (typ_subst X S T2) cs.
+Proof.
+  introv Hs Hk.
+  apply regular_subtype in Hs.
+  pose combined_kinding_typ_subst.
+  intuition eauto.
+Qed.
+
+Lemma subtype_typ_subst_l : forall E X J S T1 T2 cs,
+    subtype (E & X ~:: J) T1 T2 cs ->
+    kinding E S J ->
+    subtype E (typ_subst X S T1) (typ_subst X S T2) cs.
+Proof.
+  introv Hte Hk.
+  rewrite <- concat_empty_r with (E := E & X ~:: J) in Hte.
+  rewrite <- concat_empty_r with (E := E).
+  rewrite <- env_subst_empty with (X := X) (U := S).
+  eauto using subtype_typ_subst.
+Qed.
+
+Lemma valid_instance_typ_subst : forall E F X J S Ts M,
+  valid_instance (E & X ~:: J & F) Ts M ->
+  kinding E S J ->
+  valid_instance (E & env_subst X S F)
+       (List.map (typ_subst X S) Ts) (sch_subst X S M).
+Proof.
+  introv Hi He.
+  remember (E & X ~:: J & F) as EXF.
+  induction Hi; subst.
+  - apply valid_instance_empty.
+    fold (knd_subst X S knd_type).
+    eauto using kinding_typ_subst.
+  - apply valid_instance_bind; eauto using kinding_typ_subst.
+    fold (List.map (typ_subst X S) Ts).
+    fold (sch_subst X S M).
+    rewrite <- sch_subst_open; auto with kinding_regular.
+Qed.
+
+Lemma valid_instance_typ_subst_l : forall E X J S Ts M,
+  valid_instance (E & X ~:: J) Ts M ->
+  kinding E S J ->
+  valid_instance E (List.map (typ_subst X S) Ts) (sch_subst X S M).
+Proof.
+  introv Hv Hk.
+  rewrite <- concat_empty_r with (E := E & X ~:: J) in Hv.
+  rewrite <- concat_empty_r with (E := E).
+  rewrite <- env_subst_empty with (X := X) (U := S).
+  eauto using valid_instance_typ_subst.
+Qed.
+
+Lemma kinding_instance : forall E Ts M,
+    valid_instance E Ts M ->
+    kinding E (instance M Ts) knd_type.
+Proof.
+  introv Hi.
+  generalize dependent M.
+  induction Ts; introv Hi; destruct M; simpl;
+    inversion Hi; subst; auto.
+Qed.
 
 (* *************************************************************** *)
 (** Not affected by type bindings *)
 
-Lemma kinding_bind_typ : forall E F T K x S,
-    kinding (E & x ~: S & F) T K ->
+Lemma combined_kinding_typ_bind :
+     (forall EXF K,
+      valid_kind EXF K ->
+      (forall E F x M,
+          EXF = E & x ~: M & F ->
+          valid_kind (E & F) K))
+  /\ (forall EXF T K,
+      kinding EXF T K ->
+      (forall E F x M,
+          EXF = E & x ~: M & F ->
+          kinding (E & F) T K))
+  /\ (forall EXF Ms Xs,
+      valid_scheme_vars EXF Ms Xs ->
+      (forall E F x M,
+          EXF = E & x ~: M & F ->
+          valid_scheme_vars (E & F) Ms Xs))
+  /\ (forall EXF Ms,
+      valid_scheme EXF Ms ->
+      (forall E F x M,
+          EXF = E & x ~: M & F ->
+          valid_scheme (E & F) Ms))
+  /\ (forall EXF,
+      valid_env EXF ->
+      (forall E F x M,
+          EXF = E & x ~: M & F ->
+          valid_env (E & F)))
+  /\ (forall EXF T1 T2 K,
+      type_equal_core EXF T1 T2 K ->
+      (forall E F x M,
+          EXF = E & x ~: M & F ->
+          type_equal_core (E & F) T1 T2 K))
+  /\ (forall EXF T1 T2 K,
+      type_equal_cong EXF T1 T2 K ->
+      (forall E F x M,
+          EXF = E & x ~: M & F ->
+          type_equal_cong (E & F) T1 T2 K))
+  /\ (forall EXF T1 T2 K,
+      type_equal_symm EXF T1 T2 K ->
+      (forall E F x M,
+          EXF = E & x ~: M & F ->
+          type_equal_symm (E & F) T1 T2 K))
+  /\ (forall EXF T1 T2 K,
+      type_equal EXF T1 T2 K ->
+      (forall E F x M,
+          EXF = E & x ~: M & F ->
+          type_equal (E & F) T1 T2 K))
+  /\ (forall EXF T1 T2 cs,
+      subtype EXF T1 T2 cs ->
+      (forall E F x M,
+          EXF = E & x ~: M & F ->
+          subtype (E & F) T1 T2 cs)).
+Proof.
+  apply combined_kinding_mutind; intros; subst; simpl; econstr eauto.
+  - assert (binds X (bind_knd K) (E0 & x ~: M & F)) as Hb
+      by assumption.
+    destruct (binds_middle_inv Hb) as [? | [[? [? ?]] | [? [? ?]]]];
+      try discriminate; eauto.
+  - apply valid_scheme_vars_bind; eauto.
+    rewrite <- concat_assoc.
+    eauto using concat_assoc.
+  - exfalso. eapply empty_middle_inv. eassumption.
+  - assert (E & X ~:: K = E0 & x ~: M & F) as Heq
+      by assumption.
+    destruct F using env_ind.
+    + rewrite concat_empty_r in Heq.
+      destruct (eq_push_inv Heq) as [? [Heqb ?]].
+      discriminate.
+    + rewrite concat_assoc in Heq.
+      destruct (eq_push_inv Heq) as [? [? ?]]; subst.
+      rewrite concat_assoc.
+      apply valid_env_kind; eauto.
+  - assert (E & x ~: M = E0 & x0 ~: M0 & F) as Heq
+      by assumption.
+    destruct F using env_ind.
+    + rewrite concat_empty_r in Heq.
+      destruct (eq_push_inv Heq) as [? [Heq2 ?]].
+      inversion Heq2; subst.
+      rewrite concat_empty_r.
+      assumption.
+    + rewrite concat_assoc in Heq.
+      destruct (eq_push_inv Heq) as [? [? ?]]; subst.
+      rewrite concat_assoc.
+      apply valid_env_type; eauto.
+  - apply type_equal_core_or_associative
+      with (cs1 := cs1) (cs2 := cs2) (cs3 := cs3); eauto.
+Qed.      
+
+Lemma valid_kind_typ_bind : forall E F x M K,
+    valid_kind (E & x ~: M & F) K ->
+    valid_kind (E & F) K.
+Proof.
+  introv Hv.
+  pose combined_kinding_typ_bind.
+  intuition eauto.
+Qed.
+
+Lemma kinding_typ_bind : forall E F x M T K,
+    kinding (E & x ~: M & F) T K ->
     kinding (E & F) T K.
 Proof.
   introv Hk.
-  gen_eq Ex : (E & x ~: S & F).
-  induction Hk; intro; subst; eauto.
-  destruct (binds_middle_inv H0) as [|[[_[_ Heq]]|]]; iauto.
-  inversion Heq.
+  pose combined_kinding_typ_bind.
+  intuition eauto.
 Qed.
 
-Lemma kinding_bind_typ_l : forall E T K x S,
-    kinding (E & x ~: S) T K ->
-    kinding E T K.
+Lemma valid_scheme_vars_typ_bind : forall E F x M Ms Xs,
+    valid_scheme_vars (E & x ~: M & F) Ms Xs ->
+    valid_scheme_vars (E & F) Ms Xs.
 Proof.
-  introv Hk.
-  rewrite <- concat_empty_r with (E := E).
-  apply kinding_bind_typ with (x := x) (S := S).
-  rewrite concat_empty_r.
-  auto.
+  introv Hv.
+  pose combined_kinding_typ_bind.
+  intuition eauto.
 Qed.
 
-Lemma kindings_bind_typ : forall E F n T K x S,
-    kindings (E & x ~: S & F) n T K ->
-    kindings (E & F) n T K.
+Lemma valid_scheme_typ_bind : forall E F x M Ms,
+    valid_scheme (E & x ~: M & F) Ms ->
+    valid_scheme (E & F) Ms.
 Proof.
-  introv Hk.
-  gen_eq G : (E & x ~: S & F).
-  induction Hk; intros; subst.
-  - apply* kindings_nil.
-  - apply* kindings_cons.
-    apply kinding_bind_typ with (x := x) (S := S).
-    auto.
+  introv Hv.
+  pose combined_kinding_typ_bind.
+  intuition eauto.
 Qed.
 
-Lemma kinding_scheme_bind_typ : forall E F M x S,
-    kinding_scheme (E & x ~: S & F) M ->
-    kinding_scheme (E & F) M.
+Lemma valid_env_typ_bind : forall E F x M,
+    valid_env (E & x ~: M & F) ->
+    valid_env (E & F).
 Proof.
-  unfold kinding_scheme, kinding_body.
-  introv [L Hk].
-  exists_fresh Xs HFr.
-  destruct Hk with Xs as [Hkd Hks]; auto.
-  split; auto.
-  rewrite <- concat_assoc.
-  apply kinding_bind_typ with (x := x) (S := S).
-  rewrite concat_assoc.
-  auto.
+  introv Hv.
+  pose combined_kinding_typ_bind.
+  intuition eauto.
 Qed.
 
-Hint Resolve kinding_bind_typ : bind_typ.
-Hint Resolve kinding_bind_typ_l : bind_typ.
-Hint Resolve kindings_bind_typ : bind_typ.
-Hint Resolve kinding_scheme_bind_typ : bind_typ.
-
-(* *************************************************************** *)
-(** Preserved by type substitution *)
-
-Lemma kinding_typ_subst : forall E F X T S K J,
-  kinding (E & X ~:: J & F) T K -> 
-  kinding E S J -> 
-  kinding (E & (environment_subst X S F)) (typ_subst X S T) K.
+Lemma type_equal_core_typ_bind : forall E F x M T1 T2 K,
+    type_equal_core (E & x ~: M & F) T1 T2 K ->
+    type_equal_core (E & F) T1 T2 K.
 Proof.
-  introv Hkt Hks.
-  gen_eq G : (E & X ~:: J & F).
-  induction Hkt; introv Heq; subst; simpl typ_subst; eauto.
-  - case_var.
-    + lets Hb : (binds_middle_eq_inv H0 (ok_from_environment H)).
-      inversion Hb; subst.
-      apply* kinding_weakening_l.
-    + { apply* kinding_var.
-        - apply binds_subst_inv_r.
-          eapply binds_subst.
-          + apply H0.
-          + auto. }
+  introv Hte.
+  pose combined_kinding_typ_bind.
+  intuition eauto.
 Qed.
 
-Lemma kinding_typ_subst_l : forall E X T S K J,
-  kinding (E & X ~:: J) T K -> 
-  kinding E S J -> 
-  kinding E (typ_subst X S T) K.
+Lemma type_equal_cong_typ_bind : forall E F x M T1 T2 K,
+    type_equal_cong (E & x ~: M & F) T1 T2 K ->
+    type_equal_cong (E & F) T1 T2 K.
 Proof.
-  introv Hk1 Hk2.
-  rewrite <- concat_empty_r with (E := E).
-  rewrite <- environment_subst_empty with (X := X) (T := S).
-  apply kinding_typ_subst with (J := J); auto.
-  rewrite concat_empty_r.
-  auto.
+  introv Hte.
+  pose combined_kinding_typ_bind.
+  intuition eauto.
 Qed.
 
-Lemma kinding_typ_substs : forall E F Xs T Ss K Js n,
-  kinding (E & Xs ~::* Js & F) T K -> 
-  kindings E n Ss Js -> 
-  length Xs = n ->
-  length Js = n ->
-  length Ss = n ->
-  kinding (E & (environment_substs Xs Ss F)) (typ_substs Xs Ss T) K.
+Lemma type_equal_symm_typ_bind : forall E F x M T1 T2 K,
+    type_equal_symm (E & x ~: M & F) T1 T2 K ->
+    type_equal_symm (E & F) T1 T2 K.
 Proof.
-  intros.
-  gen Ss Js T F n.
-  induction Xs; destruct Js; destruct Ss;
-    introv Hkt Hks; intros; subst; tryfalse; rew_kinds* in Hkt.
-  inversion Hks.
-  eapply IHXs; eauto.
-  eapply kinding_typ_subst.
-  - apply Hkt.
-  - apply* kinding_weakening_l.
-    eauto using environment_concat_inv_l.
+  introv Hte.
+  pose combined_kinding_typ_bind.
+  intuition eauto.
 Qed.
 
-Lemma kinding_typ_substs_l : forall E Xs T Ss K Js n,
-  kinding (E & Xs ~::* Js) T K -> 
-  kindings E n Ss Js -> 
-  length Xs = n ->
-  length Js = n ->
-  length Ss = n ->
-  kinding E (typ_substs Xs Ss T) K.
+Lemma type_equal_typ_bind : forall E F x M T1 T2 K,
+    type_equal (E & x ~: M & F) T1 T2 K ->
+    type_equal (E & F) T1 T2 K.
 Proof.
-  introv Hk1 Hk2 Hlx Hlj Hls.
-  rewrite <- concat_empty_r with (E := E).
-  rewrite <- environment_substs_empty with (Xs := Xs) (Ts := Ss).
-  - apply kinding_typ_substs with (Js := Js) (n := n); auto.
-    rewrite concat_empty_r.
-    auto.
-  - subst*.
+  introv Hte.
+  pose combined_kinding_typ_bind.
+  intuition eauto.
 Qed.
 
-Lemma kindings_typ_subst : forall n E F X Ts S Ks J,
-  kindings (E & X ~:: J & F) n Ts Ks -> 
-  kinding E S J -> 
-  kindings (E & (environment_subst X S F)) n
-           (List.map (typ_subst X S) Ts) Ks.
+Lemma subtype_typ_bind : forall E F x M T1 T2 cs,
+    subtype (E & x ~: M & F) T1 T2 cs ->
+    subtype (E & F) T1 T2 cs.
 Proof.
-  introv Hks Hk.
-  gen_eq G : (E & X ~:: J & F).
-  induction Hks; intro; subst; simpl.
-  - apply kindings_nil.
-    destruct* (environment_kind_middle_inv H).
-  - apply kindings_cons; auto.
-    apply kinding_typ_subst with J; auto.
+  introv Hs.
+  pose combined_kinding_typ_bind.
+  intuition eauto.
 Qed.
-
-Lemma kinding_scheme_typ_subst : forall E F M X T K,
-    kinding_scheme (E & X ~:: K & F) M ->
-    kinding E T K ->
-    kinding_scheme (E & environment_subst X T F) (sch_subst X T M).
-Proof.
-  unfold kinding_scheme, kinding_body.
-  introv [L Hs] Ht.
-  exists_fresh Xs Hf.
-  unfold sch_arity in Hf.
-  lets Hlx : (fresh_length _ _ _ Hf).
-  lets Hf2 : Hf.
-  rewrite Hlx in Hf2.
-  apply fresh_length_arity_subst in Hf.
-  destruct Hs with Xs as [Hkd Hks]; auto.
-  split; auto.
-  rewrite <- concat_assoc.
-  rewrite* <- environment_subst_kinds.
-  fold (sch_open_vars (sch_subst X T M) Xs).
-  rewrite* <- sch_subst_open_vars.
-  unfold sch_open_vars.
-  apply kinding_typ_subst with (J := K); auto.
-  rewrite concat_assoc.
-  unfold sch_subst.
-  simpl.
-  apply Hs.
-  unfold sch_arity.
-  unfold sch_subst in Hf.
-  simpl in Hf.
-  auto.
-Qed.
-
-Hint Resolve kinding_typ_subst : typ_subst.
-Hint Resolve kinding_typ_subst_l : typ_subst.
-Hint Resolve kinding_typ_substs : typ_subst.
-Hint Resolve kinding_typ_substs_l : typ_subst.
-Hint Resolve kindings_typ_subst : typ_subst.
-
-Lemma kinding_sch_open : forall E M Ts,
-  kinding_scheme E M ->
-  kindings E (sch_arity M) Ts (sch_kinds M) ->
-  kinding E (sch_open M Ts) knd_type.
-Proof.
-  introv Hks Hkt.
-  destruct Hks as [L Hks].
-  pick_freshes (sch_arity M) Xs.
-  destruct Hks with Xs as [Hkd Hkk]; auto.
-  lets Hlx : (fresh_length _ _ _ Fr).
-  lets Hlk : (proj1 (proj32 (kindings_regular Hkt))).
-  rewrite* (@typ_substs_intro_sch M Xs Ts).
-  unfold sch_open_vars.
-  apply kinding_typ_substs_l
-    with (Js := sch_kinds M) (n := sch_arity M); auto.
-Qed.
-
-Hint Resolve kinding_sch_open : kinding.
  
 (* *************************************************************** *)
 (** Kinding of schemes with no parameters *)
 
-Lemma kinding_scheme_no_params : forall E T M,
-    kinding E T knd_type ->
-    M = Sch nil T ->
-    kinding_scheme E M.
+Lemma valid_scheme_empty_type : forall E T,
+    valid_scheme E (sch_empty T) <-> kinding E T knd_type.
 Proof.
-  introv Hk Heq.
-  subst.
-  exists_fresh Xs Hf.
-  simpl.
-  destruct (List.length_zero_iff_nil Xs) as [Hlz _].
-  rewrite (Hlz (eq_sym (fresh_length _ _ _ Hf))).
-  rewrite singles_nil.
-  rewrite map_empty.
-  rewrite concat_empty_r.
-  unfold typ_open_vars.
-  rewrite* <- (@typ_open_type T (typ_fvars nil)).
-Qed.
-
-(* *************************************************************** *)
-(** * Properties of well-kinded environments *)
-
-Lemma kinding_env_shorten : forall E G,
-    kinding_env (E & G) ->
-    kinding_env E.
-Proof.
-  introv Hk.
-  induction G using env_ind;
-    autorewrite with rew_env_concat in Hk; auto.
-  inversion Hk.
-  - destruct (empty_concat_inv H0) as [ He1 _ ].
-    destruct (empty_concat_inv He1) as [ He2 _ ].
-    rewrite* <- He2.
-  - destruct (eq_push_inv H) as [ _ [ _ He ] ].
-    subst*.
-  - destruct (eq_push_inv H) as [ _ [ _ He ] ].
-    subst*.
-Qed.
-
-Lemma kinding_env_kinds : forall E n Ks Xs,
-    kinding_env E ->
-    (fresh (dom E) n Xs) ->
-    kinds n Ks ->
-    kinding_env (E & Xs ~::* Ks).
-Proof.
-  introv Hk Hf Hlk.
-  lets Hlx : (eq_sym (fresh_length _ _ _ Hf)).
-  gen Ks n.
-  unfold kinds.
-  induction Xs; destruct Ks;
-    introv Hf [Hlk Hkd] Hlx; subst; tryfalse; rew_kinds*.
-  apply kinding_env_kind.
-  - apply IHXs with (length Ks); auto.
-    destruct* Hf.
-    inversion Hkd.
-    split; auto.
-  - inversion Hkd.
-    auto.
-  - eapply fresh_kinds; auto.
-Qed.
-
-Hint Resolve kinding_env_kinds : kinding.
-
-Lemma kinding_env_typ_push_inv : forall E x M,
-    kinding_env (E & x ~: M) ->
-    kinding_env E /\ x # E /\ kinding_scheme E M.
-Proof.
-  introv H.
-  inverts H as H1 H2 H3 H4.
-  - false (empty_push_inv H1).
-  - destruct (eq_push_inv H4) as [_ [Hv _]].
-    false Hv.
-  - destruct (eq_push_inv H4) as [Hx [Hv He]].
+  split.
+  - intro Hv.
+    remember (sch_empty T) as M.
+    destruct Hv; subst.
+    simpl in *.
+    assert (valid_scheme_vars E (sch_empty T) nil) as Hv by auto.
     inversion Hv.
-    subst.
-    easy.
-Qed.
-
-Lemma kinding_env_kind_push_inv : forall E x K,
-    kinding_env (E & x ~:: K) ->
-    kinding_env E /\ x # E.
-Proof.
-  introv H.
-  inverts H as H1 H2 H3 H4.
-  - false (empty_push_inv H1).
-  - destruct (eq_push_inv H4) as [Hx [_ He]].
-    subst.
-    easy.
-  - destruct (eq_push_inv H4) as [_ [Hv _]].
-    false Hv.
-Qed.
-
-Lemma kinding_scheme_from_env : forall E x M,
-    kinding_env E ->
-    binds x (bind_typ M) E ->
-    kinding_scheme E M.
-Proof.
-  introv He Hb.
-  induction E using env_ind; rew_env_concat.
-  - false (binds_empty_inv Hb).
-  - destruct (binds_push_inv Hb); jauto_set.
-    + subst.
-      destruct (kinding_env_typ_push_inv He).
-      jauto_set.
-      auto with weaken.
-    + eauto using kinding_env_shorten with weaken.
-Qed.
-
-Hint Resolve kinding_scheme_from_env : kinding.
-
-Lemma kinding_env_well_scoped : forall E F X B,
-    kinding_env (E & X ~ B & F) ->
-    X \notin (env_fv E).
-Proof.
-  introv Hkef Hfv.
-  assert (kinding_env E) as Hke by eauto using kinding_env_shorten. 
-  lets Hd : (kinding_env_closed Hke Hfv).
-  assert (ok (E & X ~ B & F)) as Hok by auto.
-  apply ok_middle_inv in Hok.
-  iauto.
+    auto.
+  - introv Hk.
+    apply valid_scheme_c with (L := typ_fv T).
+    introv Hf.
+    simpl in Hf.
+    fresh_length Hf as Hl.
+    destruct Xs; simpl in Hl; try discriminate.
+    auto.
 Qed.
 
 (* *************************************************************** *)
-(** Not affected by type bindings *)
+(** Type equality is an equivalence relation. This "raw" version
+    of the symmetry lemma requires separate evidence of the
+    well-kindedness of the types involved. A version that extracts
+    this evidence from the given relations is defined later in
+    the file. *)
 
-Lemma kinding_env_bind_typ : forall E F x M,
-    kinding_env (E & x ~: M & F) ->
-    kinding_env (E & F).
+Lemma type_equal_reflexive : forall E T K,
+    kinding E T K ->
+    type_equal E T T K.
+Proof.
+  auto.
+Qed.
+
+Lemma type_equal_transitive : forall E T1 T2 T3 K,
+    type_equal E T1 T2 K ->
+    type_equal E T2 T3 K ->
+    type_equal E T1 T3 K.
+Proof.
+  introv Hte1 Hte2.
+  induction Hte1; eauto.
+Qed.
+
+Lemma type_equal_symm_symmetric : forall E T1 T2 K,
+    type_equal_symm E T1 T2 K ->
+    type_equal_symm E T2 T1 K.
+Proof.
+  introv Hte.
+  induction Hte; auto.
+Qed.
+
+Lemma type_equal_symmetric_ind : forall E T1 T2 T3 K,
+    type_equal E T2 T1 K ->
+    type_equal E T2 T3 K ->
+    type_equal E T3 T1 K.
+Proof.
+  introv Hacc Hte.
+  induction Hte; auto.
+  eauto using type_equal_symm_symmetric.
+Qed.
+
+Lemma raw_type_equal_symmetric : forall E T1 T2 K,
+    kinding E T1 K ->
+    type_equal E T1 T2 K ->
+    type_equal E T2 T1 K.
+Proof.
+  introv Hte.
+  apply type_equal_symmetric_ind with (T2 := T1); try assumption.
+  apply type_equal_refl.
+  assumption.
+Qed.
+
+(* *************************************************************** *)
+(** The subtyping relation is a partial order. These "raw" versions
+    require separate evidence of the well-kindedness of the types
+    involved. Versions that extract this evidence from the given
+    relations are defined later in the file. *)
+
+Lemma raw_subtype_reflexive : forall E T cs,
+    valid_env E ->
+    kinding E T (knd_row cs) ->
+    subtype E T T cs.
+Proof.
+  introv Hv Hk.
+  assert (kind (knd_row cs)) as Hknd by auto with kinding_regular.
+  inversion Hknd; subst.
+  apply subtype_c.
+  apply type_equal_step
+    with (T2 := (typ_meet T (typ_join T (typ_bot cs)))); auto.
+  apply type_equal_step with (T2 := (typ_meet T T));
+    inversion Hk; subst; auto with kinding_regular.
+Qed.
+
+Lemma raw_type_equal_meet_r : forall E T1 T2 T2' cs,
+    kinding E (typ_meet T1 T2') (knd_row cs) ->
+    type_equal E T2 T2' (knd_row cs) ->
+    type_equal E (typ_meet T1 T2) (typ_meet T1 T2') (knd_row cs).
+Proof.
+  introv Hk Hte.
+  remember (knd_row cs).
+  induction Hte; subst.
+  - auto using type_equal_refl.
+  - apply type_equal_step with (T2 := typ_meet T1 T2); auto.
+    assert (type_equal_symm E T0 T2 (knd_row cs)) as Htes
+      by assumption.
+    inversion Hk.
+    remember (knd_row cs).
+    destruct Htes; subst; auto.
+Qed.
+
+Lemma raw_type_equal_meet_l : forall E T1 T1' T2 cs,
+    kinding E (typ_meet T1' T2) (knd_row cs) ->
+    type_equal E T1 T1' (knd_row cs) ->
+    type_equal E (typ_meet T1 T2) (typ_meet T1' T2) (knd_row cs).
+Proof.
+  introv Hk Hte.
+  remember (knd_row cs).
+  induction Hte; subst.
+  - auto using type_equal_refl.
+  - apply type_equal_step with (T2 := typ_meet T0 T2); auto.  
+    assert (type_equal_symm E T1 T0 (knd_row cs)) as Htes
+      by assumption.
+    inversion Hk.
+    remember (knd_row cs).
+    destruct Htes; subst; auto.
+Qed.
+      
+Lemma raw_subtype_transitive : forall E T1 T2 T3 cs,
+    kinding E T1 (knd_row cs) ->
+    kinding E T2 (knd_row cs) ->
+    kinding E T3 (knd_row cs) ->
+    subtype E T1 T2 cs ->
+    subtype E T2 T3 cs ->
+    subtype E T1 T3 cs.
+Proof.
+  introv Hk1 Hk2 Hk3 Hs1 Hs2.
+  apply subtype_c.
+  destruct Hs1. destruct Hs2.
+  apply type_equal_transitive
+    with (T2 := typ_meet T1 T0); auto.
+  apply type_equal_transitive
+    with (T2 := typ_meet T1 (typ_meet T0 T2));
+    auto using raw_type_equal_meet_r.
+  apply type_equal_step
+    with (T2 := typ_meet (typ_meet T1 T0) T2);
+    auto.
+  apply type_equal_transitive with (T2 := typ_meet T1 T2);
+    auto using raw_type_equal_meet_l, raw_type_equal_symmetric.
+Qed.
+
+Lemma raw_subtype_antisymmetric : forall E T1 T2 cs,
+    kinding E T1 (knd_row cs) ->
+    kinding E T2 (knd_row cs) ->
+    subtype E T1 T2 cs ->
+    subtype E T2 T1 cs ->
+    type_equal E T1 T2 (knd_row cs).
+Proof.
+  introv Hk1 Hk2 Hs1 Hs2.
+  destruct Hs1. destruct Hs2.
+  apply type_equal_transitive with (T2 := typ_meet T2 T1); auto.
+  apply type_equal_step with (T2 := typ_meet T1 T2); auto.
+  apply raw_type_equal_symmetric; auto.
+Qed.
+
+(* *************************************************************** *)
+(** * "Validated" versions of judgements *)
+
+Inductive valid_kind_validated : env -> knd -> Prop :=
+  | valid_kind_validated_type : forall E,
+      valid_env_validated E ->
+      environment E ->
+      valid_kind_validated E knd_type
+  | valid_kind_validated_row :  forall E cs,
+      valid_env_validated E ->
+      CSet.Nonempty cs ->
+      environment E ->
+      valid_kind_validated E (knd_row cs)
+  | valid_kind_validated_range : forall E T1 T2,
+      subtype_validated E T2 T1 CSet.universe ->
+      environment E ->
+      type T1 ->
+      type T2 ->
+      valid_env E ->
+      kinding E T1 (knd_row CSet.universe) ->
+      kinding E T2 (knd_row CSet.universe) ->
+      valid_kind_validated E (knd_range T1 T2)
+
+with kinding_validated : env -> typ -> knd -> Prop :=
+  | kinding_validated_var : forall E X K,
+      valid_env_validated E ->
+      binds X (bind_knd K) E ->
+      environment E ->
+      kind K ->
+      valid_kind E K ->
+      kinding_validated E (typ_fvar X) K
+  | kinding_validated_constructor : forall E c T cs,
+      kinding_validated E T knd_type ->
+      cs = CSet.singleton c ->
+      environment E ->
+      type T ->
+      valid_env E ->
+      kinding_validated E (typ_constructor c T) (knd_row cs)
+  | kinding_validated_or : forall E T1 T2 cs1 cs2 cs12,
+      kinding_validated E T1 (knd_row cs1) ->
+      kinding_validated E T2 (knd_row cs2) ->
+      CSet.Disjoint cs1 cs2 ->
+      cs12 = CSet.union cs1 cs2 ->
+      environment E ->
+      type T1 ->
+      type T2 ->
+      CSet.Nonempty cs1 ->
+      CSet.Nonempty cs2 ->
+      valid_env E ->
+      kinding_validated E (typ_or T1 T2) (knd_row cs12)
+  | kinding_validated_proj : forall E T cs cs',
+      kinding_validated E T (knd_row cs) ->
+      CSet.Subset cs' cs ->
+      CSet.Nonempty cs' ->
+      environment E ->
+      type T ->
+      CSet.Nonempty cs ->
+      valid_env E ->
+      kinding_validated E (typ_proj T cs') (knd_row cs')
+  | kinding_validated_row : forall E T,
+      kinding_validated E T (knd_row CSet.universe) ->
+      environment E ->
+      type T ->
+      valid_env E ->
+      kinding_validated E (typ_row T) (knd_range T T)
+  | kinding_validated_variant : forall E T T1 T2,
+      kinding_validated E T (knd_range T1 T2) ->
+      environment E ->
+      type T ->
+      type T1 ->
+      type T2 ->
+      valid_env E ->
+      kinding E T1 (knd_row CSet.universe) ->
+      kinding E T2 (knd_row CSet.universe) ->
+      subtype E T2 T1 CSet.universe ->
+      kinding_validated E (typ_variant T) knd_type
+  | kinding_validated_arrow : forall E T1 T2,
+      kinding_validated E T1 knd_type -> 
+      kinding_validated E T2 knd_type -> 
+      environment E ->
+      type T1 ->
+      type T2 ->
+      valid_env E ->
+      kinding_validated E (typ_arrow T1 T2) knd_type
+  | kinding_validated_top : forall E cs,
+      valid_env_validated E ->
+      CSet.Nonempty cs ->
+      environment E ->
+      valid_env E ->
+      kinding_validated E (typ_top cs) (knd_row cs)
+  | kinding_validated_bot : forall E cs,
+      valid_env_validated E ->
+      CSet.Nonempty cs ->
+      environment E ->
+      valid_env E ->
+      kinding_validated E (typ_bot cs) (knd_row cs)
+  | kinding_validated_meet : forall E T1 T2 cs,
+      kinding_validated E T1 (knd_row cs) ->
+      kinding_validated E T2 (knd_row cs) ->
+      environment E ->
+      type T1 ->
+      type T2 ->
+      CSet.Nonempty cs ->
+      valid_env E ->
+      kinding_validated E (typ_meet T1 T2) (knd_row cs)
+  | kinding_validated_join : forall E T1 T2 cs,
+      kinding_validated E T1 (knd_row cs) ->
+      kinding_validated E T2 (knd_row cs) ->
+      environment E ->
+      type T1 ->
+      type T2 ->
+      CSet.Nonempty cs ->
+      valid_env E ->
+      kinding_validated E (typ_join T1 T2) (knd_row cs)
+  | kinding_validated_range_subsumption : forall E T T1 T2 T1' T2',
+      kinding_validated E T (knd_range T1 T2) ->
+      subtype_validated E T1 T1' CSet.universe ->
+      subtype_validated E T2' T2 CSet.universe ->
+      environment E ->
+      type T ->
+      type T1 ->
+      type T2 ->
+      type T1' ->
+      type T2' ->
+      valid_env E ->
+      kinding E T1 (knd_row CSet.universe) ->
+      kinding E T1' (knd_row CSet.universe) ->
+      kinding E T2 (knd_row CSet.universe) ->
+      kinding E T2' (knd_row CSet.universe) ->
+      subtype E T2 T1 CSet.universe ->
+      subtype E T2' T1' CSet.universe ->
+      kinding_validated E T (knd_range T1' T2')
+
+with valid_scheme_vars_validated : env -> sch -> list var -> Prop :=
+  | valid_scheme_vars_validated_empty : forall E T,
+      kinding_validated E T knd_type ->
+      environment E ->
+      type T ->
+      valid_env E ->
+      valid_scheme_vars_validated E (sch_empty T) nil
+  | valid_scheme_vars_validated_bind : forall X Xs E K M,
+      valid_kind_validated E K ->
+      valid_scheme_vars_validated (E & X ~:: K) (M ^ X) Xs ->
+      environment E ->
+      environment (E & X ~:: K) ->
+      kind K ->
+      scheme_vars (M ^ X) Xs ->
+      scheme_vars (sch_bind K M) (X :: Xs) ->
+      valid_env E ->
+      valid_env (E & X ~:: K) ->
+      valid_scheme_vars_validated E (sch_bind K M) (X :: Xs)
+
+with valid_scheme_validated : env -> sch -> Prop :=
+  | valid_scheme_validated_c : forall E M L,
+      (forall Xs,
+          fresh L (sch_arity M) Xs ->
+          valid_scheme_vars_validated E M Xs) ->
+      environment E ->
+      scheme M ->
+      valid_env E ->
+      valid_scheme_validated E M
+
+with valid_env_validated : env -> Prop :=
+  | valid_env_validated_empty :
+      valid_env_validated empty
+  | valid_env_validated_kind : forall E X K,
+      valid_env_validated E ->
+      valid_kind_validated E K ->
+      X # E ->
+      environment E ->
+      environment (E & X ~:: K) ->
+      kind K ->
+      valid_env_validated (E & X ~:: K)
+  | valid_env_validated_type : forall E x M,
+      valid_env_validated E ->
+      valid_scheme_validated E M ->
+      x # E ->
+      environment E ->
+      environment (E & x ~: M) ->
+      scheme M ->
+      valid_env_validated (E & x ~: M)
+
+with type_equal_core_validated : env -> typ -> typ -> knd -> Prop :=
+  | type_equal_core_validated_or_commutative :
+      forall E T1 T2 cs1 cs2 cs12,
+      kinding_validated E T1 (knd_row cs1) ->
+      kinding_validated E T2 (knd_row cs2) ->
+      CSet.Disjoint cs1 cs2 ->
+      cs12 = CSet.union cs1 cs2 ->
+      environment E ->
+      type T1 ->
+      type T2 ->
+      CSet.Nonempty cs1 ->
+      CSet.Nonempty cs2 ->
+      valid_env E ->
+      type_equal_core_validated E
+        (typ_or T1 T2) (typ_or T2 T1) (knd_row cs12)
+  | type_equal_core_validated_or_associative :
+      forall E T1 cs1 T2 cs2 T3 cs3 cs123,
+      kinding_validated E T1 (knd_row cs1) ->
+      kinding_validated E T2 (knd_row cs2) ->
+      kinding_validated E T3 (knd_row cs3) ->
+      CSet.Disjoint cs1 cs2 ->
+      CSet.Disjoint cs1 cs3 ->
+      CSet.Disjoint cs2 cs3 ->
+      cs123 = CSet.union cs1 (CSet.union cs2 cs3) ->
+      environment E ->
+      type T1 ->
+      type T2 ->
+      type T3 ->
+      CSet.Nonempty cs1 ->
+      CSet.Nonempty cs2 ->
+      CSet.Nonempty cs3 ->
+      valid_env E ->
+      type_equal_core_validated E
+        (typ_or T1 (typ_or T2 T3)) (typ_or (typ_or T1 T2) T3)
+        (knd_row cs123)
+  | type_equal_core_validated_or_bot : forall E cs1 cs2 cs12,
+      valid_env_validated E ->
+      CSet.Nonempty cs1 ->
+      CSet.Nonempty cs2 ->
+      CSet.Disjoint cs1 cs2 ->
+      cs12 = CSet.union cs1 cs2 ->
+      environment E ->
+      type_equal_core_validated E
+        (typ_or (typ_bot cs1) (typ_bot cs2)) (typ_bot cs12)
+        (knd_row cs12)
+  | type_equal_core_validated_or_top : forall E cs1 cs2 cs12,
+      valid_env_validated E ->
+      CSet.Nonempty cs1 ->
+      CSet.Nonempty cs2 ->
+      CSet.Disjoint cs1 cs2 ->
+      cs12 = CSet.union cs1 cs2 ->
+      environment E ->
+      type_equal_core_validated E
+        (typ_or (typ_top cs1) (typ_top cs2)) (typ_top cs12)
+        (knd_row cs12)
+  | type_equal_core_validated_or_meet_distribution :
+      forall E T1 T2 T3 T4 cs1 cs2 cs12,
+      kinding_validated E T1 (knd_row cs1) ->
+      kinding_validated E T2 (knd_row cs2) ->
+      kinding_validated E T3 (knd_row cs1) ->
+      kinding_validated E T4 (knd_row cs2) ->
+      CSet.Disjoint cs1 cs2 ->
+      cs12 = CSet.union cs1 cs2 ->
+      environment E ->
+      type T1 ->
+      type T2 ->
+      type T3 ->
+      type T4 ->
+      CSet.Nonempty cs1 ->
+      CSet.Nonempty cs2 ->
+      valid_env E ->
+      type_equal_core_validated E
+        (typ_or (typ_meet T1 T3) (typ_meet T2 T4))
+        (typ_meet (typ_or T1 T2) (typ_or T3 T4))
+        (knd_row cs12)
+  | type_equal_core_validated_or_join_distribution :
+      forall E T1 T2 T3 T4 cs1 cs2 cs12,
+      kinding_validated E T1 (knd_row cs1) ->
+      kinding_validated E T2 (knd_row cs2) ->
+      kinding_validated E T3 (knd_row cs1) ->
+      kinding_validated E T4 (knd_row cs2) ->
+      CSet.Disjoint cs1 cs2 ->
+      cs12 = CSet.union cs1 cs2 ->
+      environment E ->
+      type T1 ->
+      type T2 ->
+      type T3 ->
+      type T4 ->
+      CSet.Nonempty cs1 ->
+      CSet.Nonempty cs2 ->
+      valid_env E ->
+      type_equal_core_validated E
+        (typ_or (typ_join T1 T3) (typ_join T2 T4))
+        (typ_join (typ_or T1 T2) (typ_or T3 T4))
+        (knd_row cs12)
+  | type_equal_core_validated_or_proj : forall E T cs1 cs2 cs3 cs23,
+      kinding_validated E T (knd_row cs1) ->
+      CSet.Disjoint cs2 cs3 ->
+      CSet.Subset cs2 cs1 ->
+      CSet.Nonempty cs2 ->
+      CSet.Subset cs3 cs1 ->
+      CSet.Nonempty cs3 ->
+      cs23 = CSet.union cs2 cs3 ->
+      environment E ->
+      type T ->
+      CSet.Nonempty cs1 ->
+      valid_env E ->
+      type_equal_core_validated E
+        (typ_or (typ_proj T cs2) (typ_proj T cs3))
+        (typ_proj T cs23)
+        (knd_row cs23)
+  | type_equal_core_validated_proj_id : forall E T cs,
+      kinding_validated E T (knd_row cs) ->
+      environment E ->
+      type T ->
+      CSet.Nonempty cs ->
+      valid_env E ->
+      type_equal_core_validated E (typ_proj T cs) T (knd_row cs)
+  | type_equal_core_validated_proj_or_l : forall E T1 T2 cs1 cs1' cs2,
+      kinding_validated E T1 (knd_row cs1) ->
+      kinding_validated E T2 (knd_row cs2) ->
+      CSet.Disjoint cs1 cs2 ->
+      CSet.Subset cs1' cs1 ->
+      CSet.Nonempty cs1' ->
+      environment E ->
+      type T1 ->
+      type T2 ->
+      CSet.Nonempty cs1 ->
+      CSet.Nonempty cs2 ->
+      valid_env E ->
+      type_equal_core_validated E
+        (typ_proj (typ_or T1 T2) cs1') (typ_proj T1 cs1')
+        (knd_row cs1')
+  | type_equal_core_validated_proj_or_r : forall E T1 T2 cs1 cs2 cs2',
+      kinding_validated E T1 (knd_row cs1) ->
+      kinding_validated E T2 (knd_row cs2) ->
+      CSet.Disjoint cs1 cs2 ->
+      CSet.Subset cs2' cs2 ->
+      CSet.Nonempty cs2' ->
+      environment E ->
+      type T1 ->
+      type T2 ->
+      CSet.Nonempty cs1 ->
+      CSet.Nonempty cs2 ->
+      valid_env E ->
+      type_equal_core_validated E
+        (typ_proj (typ_or T1 T2) cs2') (typ_proj T2 cs2')
+        (knd_row cs2')
+  | type_equal_core_validated_proj_or_both :
+      forall E T1 T2 cs1 cs2 cs1' cs2' cs12',
+      kinding_validated E T1 (knd_row cs1) ->
+      kinding_validated E T2 (knd_row cs2) ->
+      CSet.Disjoint cs1 cs2 ->
+      CSet.Subset cs1' cs1 ->
+      CSet.Nonempty cs1' ->
+      CSet.Subset cs2' cs2 ->
+      CSet.Nonempty cs2' ->
+      cs12' = CSet.union cs1' cs2' ->
+      environment E ->
+      type T1 ->
+      type T2 ->
+      CSet.Nonempty cs1 ->
+      CSet.Nonempty cs2 ->
+      valid_env E ->
+      type_equal_core_validated E
+        (typ_proj (typ_or T1 T2) cs12')
+        (typ_or (typ_proj T1 cs1') (typ_proj T2 cs2'))
+        (knd_row cs12')
+  | type_equal_core_validated_proj_meet : forall E T1 T2 cs cs',
+      kinding_validated E T1 (knd_row cs) ->
+      kinding_validated E T2 (knd_row cs) ->
+      CSet.Subset cs' cs ->
+      CSet.Nonempty cs' ->
+      environment E ->
+      type T1 ->
+      type T2 ->
+      CSet.Nonempty cs ->
+      valid_env E ->
+      type_equal_core_validated E
+        (typ_proj (typ_meet T1 T2) cs')
+        (typ_meet (typ_proj T1 cs') (typ_proj T2 cs'))
+        (knd_row cs')
+  | type_equal_core_validated_proj_join : forall E T1 T2 cs cs',
+      kinding_validated E T1 (knd_row cs) ->
+      kinding_validated E T2 (knd_row cs) ->
+      CSet.Subset cs' cs ->
+      CSet.Nonempty cs' ->
+      environment E ->
+      type T1 ->
+      type T2 ->
+      CSet.Nonempty cs ->
+      valid_env E ->
+      type_equal_core_validated E
+        (typ_proj (typ_join T1 T2) cs')
+        (typ_join (typ_proj T1 cs') (typ_proj T2 cs'))
+        (knd_row cs')
+  | type_equal_core_validated_meet_commutative : forall E T1 T2 cs,
+      kinding_validated E T1 (knd_row cs) ->
+      kinding_validated E T2 (knd_row cs) ->
+      environment E ->
+      type T1 ->
+      type T2 ->
+      CSet.Nonempty cs ->
+      valid_env E ->
+      type_equal_core_validated E
+        (typ_meet T1 T2) (typ_meet T2 T1) (knd_row cs)
+  | type_equal_core_validated_meet_associative : forall E T1 T2 T3 cs,
+      kinding_validated E T1 (knd_row cs) ->
+      kinding_validated E T2 (knd_row cs) ->
+      kinding_validated E T3 (knd_row cs) ->
+      environment E ->
+      type T1 ->
+      type T2 ->
+      type T3 ->
+      CSet.Nonempty cs ->
+      valid_env E ->
+      type_equal_core_validated E
+        (typ_meet T1 (typ_meet T2 T3))
+        (typ_meet (typ_meet T1 T2) T3)
+        (knd_row cs)
+  | type_equal_core_validated_meet_identity : forall E T1 cs,
+      kinding_validated E T1 (knd_row cs) ->
+      environment E ->
+      type T1 ->
+      CSet.Nonempty cs ->
+      valid_env E ->
+      type_equal_core_validated E
+        (typ_meet T1 (typ_top cs)) T1 (knd_row cs)
+  | type_equal_core_validated_meet_absorption : forall E T1 T2 cs,
+      kinding_validated E T1 (knd_row cs) ->
+      kinding_validated E T2 (knd_row cs) ->
+      environment E ->
+      type T1 ->
+      type T2 ->
+      CSet.Nonempty cs ->
+      valid_env E ->
+      type_equal_core_validated E
+        (typ_meet T1 (typ_join T1 T2)) T1 (knd_row cs)
+  | type_equal_core_validated_meet_distribution :
+      forall E T1 T2 T3 cs,
+      kinding_validated E T1 (knd_row cs) ->
+      kinding_validated E T2 (knd_row cs) ->
+      kinding_validated E T3 (knd_row cs) ->
+      environment E ->
+      type T1 ->
+      type T2 ->
+      type T3 ->
+      CSet.Nonempty cs ->
+      valid_env E ->
+      type_equal_core_validated E
+        (typ_meet T1 (typ_join T2 T3))
+        (typ_join (typ_meet T1 T2) (typ_meet T1 T3))
+        (knd_row cs)
+  | type_equal_core_validated_join_commutative : forall E T1 T2 cs,
+      kinding_validated E T1 (knd_row cs) ->
+      kinding_validated E T2 (knd_row cs) ->
+      environment E ->
+      type T1 ->
+      type T2 ->
+      CSet.Nonempty cs ->
+      valid_env E ->
+      type_equal_core_validated E
+        (typ_join T1 T2) (typ_join T2 T1) (knd_row cs)
+  | type_equal_core_validated_join_associative : forall E T1 T2 T3 cs,
+      kinding_validated E T1 (knd_row cs) ->
+      kinding_validated E T2 (knd_row cs) ->
+      kinding_validated E T3 (knd_row cs) ->
+      environment E ->
+      type T1 ->
+      type T2 ->
+      type T3 ->
+      CSet.Nonempty cs ->
+      valid_env E ->
+      type_equal_core_validated E
+        (typ_join T1 (typ_join T2 T3))
+        (typ_join (typ_join T1 T2) T3)
+        (knd_row cs)
+  | type_equal_core_validated_join_identity : forall E T1 cs,
+      kinding_validated E T1 (knd_row cs) ->
+      environment E ->
+      type T1 ->
+      CSet.Nonempty cs ->
+      valid_env E ->
+      type_equal_core_validated E
+        (typ_join T1 (typ_bot cs)) T1 (knd_row cs)
+  | type_equal_core_validated_join_absorption : forall E T1 T2 cs,
+      kinding_validated E T1 (knd_row cs) ->
+      kinding_validated E T2 (knd_row cs) ->
+      environment E ->
+      type T1 ->
+      type T2 ->
+      CSet.Nonempty cs ->
+      valid_env E ->
+      type_equal_core_validated E
+        (typ_join T1 (typ_meet T1 T2)) T1 (knd_row cs)
+  | type_equal_core_validated_join_distribution :
+      forall E T1 T2 T3 cs,
+      kinding_validated E T1 (knd_row cs) ->
+      kinding_validated E T2 (knd_row cs) ->
+      kinding_validated E T3 (knd_row cs) ->
+      environment E ->
+      type T1 ->
+      type T2 ->
+      type T3 ->
+      CSet.Nonempty cs ->
+      valid_env E ->
+      type_equal_core_validated E
+        (typ_join T1 (typ_meet T2 T3))
+        (typ_meet (typ_join T1 T2) (typ_join T1 T3))
+        (knd_row cs)
+
+with type_equal_cong_validated : env -> typ -> typ -> knd -> Prop :=
+  | type_equal_cong_validated_constructor : forall E c T1 T1' cs,
+      type_equal_cong_validated E T1 T1' knd_type ->
+      cs = CSet.singleton c ->
+      environment E ->
+      type T1 ->
+      type T1' ->
+      valid_env E ->
+      kinding E T1 knd_type ->
+      kinding E T1' knd_type ->
+      type_equal_cong_validated E
+        (typ_constructor c T1) (typ_constructor c T1')
+        (knd_row cs)
+  | type_equal_cong_validated_or_l : forall E T1 T1' T2 cs1 cs2 cs12,
+      kinding_validated E T2 (knd_row cs2) ->
+      CSet.Disjoint cs1 cs2 ->
+      cs12 = CSet.union cs1 cs2 ->
+      type_equal_cong_validated E T1 T1' (knd_row cs1) ->
+      environment E ->
+      type T1 ->
+      type T1' ->
+      type T2 ->
+      CSet.Nonempty cs1 ->
+      CSet.Nonempty cs2 ->
+      valid_env E ->
+      kinding E T1 (knd_row cs1) ->
+      kinding E T1' (knd_row cs1) ->
+      type_equal_cong_validated E
+        (typ_or T1 T2) (typ_or T1' T2) (knd_row cs12)
+  | type_equal_cong_validated_or_r : forall E T1 T2 T2' cs1 cs2 cs12,
+      kinding_validated E T1 (knd_row cs1) ->
+      CSet.Disjoint cs1 cs2 ->
+      cs12 = CSet.union cs1 cs2 ->
+      type_equal_cong_validated E T2 T2' (knd_row cs2) ->
+      environment E ->
+      type T1 ->
+      type T2 ->
+      type T2' ->
+      CSet.Nonempty cs1 ->
+      CSet.Nonempty cs2 ->
+      valid_env E ->
+      kinding E T2 (knd_row cs2) ->
+      kinding E T2' (knd_row cs2) ->
+      type_equal_cong_validated E
+        (typ_or T1 T2) (typ_or T1 T2') (knd_row cs12)
+  | type_equal_cong_validated_row : forall E T1 T1',
+      type_equal_cong_validated E T1 T1' (knd_row CSet.universe) ->
+      environment E ->
+      type T1 ->
+      type T1' ->
+      valid_env E ->
+      kinding E T1 (knd_row CSet.universe) ->
+      kinding E T1' (knd_row CSet.universe) ->
+      type_equal_cong_validated E
+        (typ_row T1) (typ_row T1') (knd_range T1 T1)
+  | type_equal_cong_validated_variant : forall E T1 T1' T2 T3,
+      type_equal_cong_validated E T1 T1' (knd_range T2 T3) ->
+      environment E ->
+      type T1 ->
+      type T1' ->
+      type T2 ->
+      type T3 ->
+      valid_env E ->
+      kinding E T1 (knd_range T2 T3) ->
+      kinding E T1' (knd_range T2 T3) ->
+      kinding E T2 (knd_row CSet.universe) ->
+      kinding E T3 (knd_row CSet.universe) ->
+      subtype E T3 T2 CSet.universe ->
+      type_equal_cong_validated E
+        (typ_variant T1) (typ_variant T1') (knd_range T2 T3)
+  | type_equal_cong_validated_arrow_l : forall E T1 T1' T2,
+      kinding_validated E T2 knd_type ->
+      type_equal_cong_validated E T1 T1' knd_type ->
+      environment E ->
+      type T1 ->
+      type T1' ->
+      type T2 ->
+      valid_env E ->
+      kinding E T1 knd_type ->
+      kinding E T1' knd_type ->
+      type_equal_cong_validated E
+        (typ_arrow T1 T2) (typ_arrow T1' T2) knd_type
+  | type_equal_cong_validated_arrow_r : forall E T1 T2 T2',
+      kinding_validated E T1 knd_type ->
+      type_equal_cong_validated E T2 T2' knd_type ->
+      environment E ->
+      type T1 ->
+      type T2 ->
+      type T2' ->
+      valid_env E ->
+      kinding E T2 knd_type ->
+      kinding E T2' knd_type ->
+      type_equal_cong_validated E
+        (typ_arrow T1 T2) (typ_arrow T1 T2') knd_type
+  | type_equal_cong_validated_meet_l : forall E T1 T1' T2 cs,
+      kinding_validated E T2 (knd_row cs) ->
+      type_equal_cong_validated E T1 T1' (knd_row cs) ->
+      environment E ->
+      type T1 ->
+      type T1' ->
+      type T2 ->
+      CSet.Nonempty cs ->
+      valid_env E ->
+      kinding E T1 (knd_row cs) ->
+      kinding E T1' (knd_row cs) ->
+      type_equal_cong_validated E
+        (typ_meet T1 T2) (typ_meet T1' T2) (knd_row cs)
+  | type_equal_cong_validated_meet_r : forall E T1 T2 T2' cs,
+      kinding_validated E T1 (knd_row cs) ->
+      type_equal_cong_validated E T2 T2' (knd_row cs) -> 
+      environment E ->
+      type T1 ->
+      type T2 ->
+      type T2' ->
+      CSet.Nonempty cs ->
+      valid_env E ->
+      kinding E T2 knd_type ->
+      kinding E T2' knd_type ->
+      type_equal_cong_validated E
+        (typ_meet T1 T2) (typ_meet T1 T2') (knd_row cs)
+  | type_equal_cong_validated_join_l : forall E T1 T1' T2 cs,
+      kinding_validated E T2 (knd_row cs) ->
+      type_equal_cong_validated E T1 T1' (knd_row cs) ->
+      environment E ->
+      type T1 ->
+      type T1' ->
+      type T2 ->
+      CSet.Nonempty cs ->
+      valid_env E ->
+      kinding E T1 knd_type ->
+      kinding E T1' knd_type ->
+      type_equal_cong_validated E
+        (typ_join T1 T2) (typ_join T1' T2) (knd_row cs)
+  | type_equal_cong_validated_join_r : forall E T1 T2 T2' cs,
+      kinding_validated E T1 (knd_row cs) ->
+      type_equal_cong_validated E T2 T2' (knd_row cs) ->
+      environment E ->
+      type T1 ->
+      type T2 ->
+      type T2' ->
+      CSet.Nonempty cs ->
+      valid_env E ->
+      kinding E T2 knd_type ->
+      kinding E T2' knd_type ->
+      type_equal_cong_validated E
+        (typ_join T1 T2) (typ_join T1 T2') (knd_row cs)
+  | type_equal_cong_validated_range_subsumption :
+      forall E T1 T2 T3 T4 T3' T4',
+      type_equal_cong_validated E T1 T2 (knd_range T3 T4) ->
+      subtype_validated E T3 T3' CSet.universe ->
+      subtype_validated E T4' T4 CSet.universe ->
+      environment E ->
+      type T1 ->
+      type T2 ->
+      type T3 ->
+      type T3' ->
+      type T4 ->
+      type T4' ->
+      valid_env E ->
+      kinding E T1 (knd_range T3 T4) ->
+      kinding E T2 (knd_range T3 T4) ->
+      kinding E T3 (knd_row CSet.universe) ->
+      kinding E T3' (knd_row CSet.universe) ->
+      kinding E T4 (knd_row CSet.universe) ->
+      kinding E T4' (knd_row CSet.universe) ->
+      subtype E T4 T3 CSet.universe ->
+      subtype E T4' T3' CSet.universe ->
+      type_equal_cong_validated E T1 T2 (knd_range T3' T4')
+  | type_equal_cong_validated_core : forall E T1 T1' K,
+      type_equal_core_validated E T1 T1' K ->
+      environment E ->
+      type T1 ->
+      type T1' ->
+      kind K ->
+      valid_env E ->
+      kinding E T1 K ->
+      kinding E T1' K ->
+      valid_kind E K ->
+      type_equal_cong_validated E T1 T1' K
+
+with type_equal_symm_validated : env -> typ -> typ -> knd -> Prop :=
+  | type_equal_symm_validated_l : forall E T1 T2 K,
+      type_equal_cong_validated E T1 T2 K ->
+      environment E ->
+      type T1 ->
+      type T2 ->
+      kind K ->
+      valid_env E ->
+      kinding E T1 K ->
+      kinding E T2 K ->
+      valid_kind E K ->
+      type_equal_symm_validated E T1 T2 K
+  | type_equal_symm_validated_r : forall E T1 T2 K,
+      type_equal_cong_validated E T1 T2 K ->
+      environment E ->
+      type T1 ->
+      type T2 ->
+      kind K ->
+      valid_env E ->
+      kinding E T1 K ->
+      kinding E T2 K ->
+      valid_kind E K ->
+      type_equal_symm_validated E T2 T1 K
+
+with type_equal_validated : env -> typ -> typ -> knd -> Prop :=
+  | type_equal_validated_refl : forall E T K,
+      kinding_validated E T K ->
+      environment E ->
+      type T ->
+      kind K ->
+      valid_env E ->
+      valid_kind E K ->
+      type_equal_validated E T T K
+  | type_equal_validated_step : forall E T1 T2 T3 K,
+      type_equal_symm_validated E T1 T2 K ->
+      type_equal_validated E T2 T3 K ->
+      environment E ->
+      type T1 ->
+      type T2 ->
+      type T3 ->
+      kind K ->
+      valid_env E ->
+      kinding E T1 K ->
+      kinding E T2 K ->
+      kinding E T3 K ->
+      valid_kind E K ->
+      type_equal_validated E T1 T3 K
+
+with subtype_validated : env -> typ -> typ -> cset -> Prop :=
+  | subtype_validated_c : forall E T1 T2 cs,
+      type_equal_validated E T1 (typ_meet T1 T2) (knd_row cs) ->
+      environment E ->
+      type T1 ->
+      type T2 ->
+      CSet.Nonempty cs ->
+      valid_env E ->
+      kinding E T1 (knd_row cs) ->
+      kinding E T2 (knd_row cs) ->
+      subtype_validated E T1 T2 cs.
+
+Scheme valid_kind_validated_mutind :=
+         Induction for valid_kind_validated Sort Prop
+  with kinding_validated_mutind :=
+         Induction for kinding_validated Sort Prop
+  with valid_scheme_vars_validated_mutind :=
+         Induction for valid_scheme_vars_validated Sort Prop
+  with valid_scheme_validated_mutind :=
+         Induction for valid_scheme_validated Sort Prop
+  with valid_env_validated_mutind :=
+         Induction for valid_env_validated Sort Prop
+  with type_equal_core_validated_mutind :=
+         Induction for type_equal_core_validated Sort Prop
+  with type_equal_cong_validated_mutind :=
+         Induction for type_equal_cong_validated Sort Prop
+  with type_equal_symm_validated_mutind :=
+         Induction for type_equal_symm_validated Sort Prop
+  with type_equal_validated_mutind :=
+         Induction for type_equal_validated Sort Prop
+  with subtype_validated_mutind :=
+         Induction for subtype_validated Sort Prop.
+
+Combined Scheme combined_kinding_validated_mutind
+  from valid_kind_validated_mutind, kinding_validated_mutind,
+       valid_scheme_vars_validated_mutind, valid_scheme_validated_mutind,
+       valid_env_validated_mutind, type_equal_core_validated_mutind,
+       type_equal_cong_validated_mutind, type_equal_symm_validated_mutind,
+       type_equal_validated_mutind, subtype_validated_mutind.
+
+Lemma valid_kind_validated_inv : forall E K,
+    valid_kind_validated E K ->
+    environment E /\ kind K.
+Proof.
+  introv Hv.
+  destruct Hv; auto.
+Qed.
+
+Hint Constructors valid_kind_validated : valid_kind_validated.
+
+Hint Extern 1 (environment ?E) =>
+  match goal with
+  | H : valid_kind_validated E _ |- _ =>
+      apply (proj1 (valid_kind_validated_inv H))
+  end : valid_kind_validated.
+
+Hint Extern 1 (kind ?K) =>
+  match goal with
+  | H : valid_kind_validated _ K |- _ =>
+      apply (proj2 (valid_kind_validated_inv H))
+  end : valid_kind_validated.
+
+Hint Extern 1 (CSet.Nonempty ?cs) =>
+  match goal with
+  | H : valid_kind_validated _ (knd_row cs) |- _ =>
+      let Hknd := fresh "Hknd" in
+      assert (kind (knd_row cs)) as Hknd
+        by apply (proj2 (valid_kind_validated_inv H));
+      inversion Hknd; assumption
+  end : valid_kind_validated.
+
+Lemma kinding_validated_inv : forall E T K,
+    kinding_validated E T K ->
+    environment E /\ type T /\ kind K.
 Proof.
   introv Hk.
-  induction F using env_ind.
-  - rewrite concat_empty_r.
-    eauto using kinding_env_shorten.
-  - rewrite concat_assoc in *.
-    inversion Hk.
-    + apply empty_push_inv in H0.
-      tryfalse.
-    + destruct (eq_push_inv H) as [Ha [Hb Hc]].
-      subst.
-      apply kinding_env_kind; auto.
-    + destruct (eq_push_inv H) as [Ha [Hb Hc]].
-      subst; eauto using kinding_scheme_bind_typ.
+  destruct Hk; auto with csetdec.
 Qed.
 
-Hint Resolve kinding_env_bind_typ : bind_typ.
+Hint Constructors kinding_validated : kinding_validated.
+
+Hint Extern 1 (environment ?E) =>
+  match goal with
+  | H : kinding_validated E _ _ |- _ =>
+      apply (proj31 (kinding_validated_inv H))
+  end : kinding_validated.
+
+Hint Extern 1 (type ?T) =>
+  match goal with
+  | H : kinding_validated _ T _ |- _ =>
+      apply (proj32 (kinding_validated_inv H))
+  end : kinding_validated.
+
+Hint Extern 1 (kind ?K) =>
+  match goal with
+  | H : kinding_validated _ _ K |- _ =>
+      apply (proj33 (kinding_validated_inv H))
+  end : kinding_validated.
+
+Hint Extern 1 (CSet.Nonempty ?cs) =>
+  match goal with
+  | H : kinding_validated _ _ (knd_row cs) |- _ =>
+      let Hknd := fresh "Hknd" in
+      assert (kind (knd_row cs)) as Hknd
+        by apply (proj33 (kinding_validated_inv H));
+      inversion Hknd; assumption
+  end : kinding_validated.
+
+Lemma valid_scheme_vars_validated_inv : forall E M Xs,
+    valid_scheme_vars_validated E M Xs ->
+    environment E /\ scheme_vars M Xs.
+Proof.
+  introv Hs.
+  destruct Hs; auto.
+Qed.
+
+Hint Constructors valid_scheme_vars_validated
+  : valid_scheme_vars_validated.
+
+Hint Extern 1 (environment ?E) =>
+  match goal with
+  | H : valid_scheme_vars_validated E _ _ |- _ =>
+      apply (proj1 (valid_scheme_vars_validated_inv H))
+  end : valid_scheme_vars_validated.
+
+Hint Extern 1 (scheme_vars ?M ?Xs) =>
+  match goal with
+  | H : valid_scheme_vars_validated _ M Xs |- _ =>
+      apply (proj2 (valid_scheme_vars_validated_inv H))
+  end : valid_scheme_vars_validated.
+
+Lemma valid_scheme_validated_inv : forall E M,
+    valid_scheme_validated E M ->
+    environment E /\ scheme M.
+Proof.
+  introv Hs.
+  destruct Hs; auto.
+Qed.
+
+Hint Constructors valid_scheme_validated : valid_scheme_validated.
+
+Hint Extern 1 (environment ?E) =>
+  match goal with
+  | H : valid_scheme_validated E _ |- _ =>
+      apply (proj1 (valid_scheme_validated_inv H))
+  end : valid_scheme_validated.
+
+Hint Extern 1 (scheme ?M) =>
+  match goal with
+  | H : valid_scheme_validated _ M |- _ =>
+      apply (proj2 (valid_scheme_validated_inv H))
+  end : valid_scheme_validated.
+
+Lemma valid_env_validated_inv : forall E,
+    valid_env_validated E -> environment E.
+Proof.
+  introv He.
+  destruct He; auto.
+Qed.
+
+Hint Constructors valid_env_validated : valid_env_validated.
+
+Hint Extern 1 (environment ?E) =>
+  match goal with
+  | H : valid_env_validated E |- _ =>
+      apply (valid_env_validated_inv H)
+  end : valid_env_validated.
+
+Lemma type_equal_core_validated_inv : forall E T1 T2 K,
+    type_equal_core_validated E T1 T2 K ->
+    environment E /\ type T1 /\ type T2 /\ kind K.
+Proof.
+  introv Hte.
+  destruct Hte; subst; split; auto with csetdec.
+Qed.
+
+Hint Constructors type_equal_core_validated : type_equal_core_validated.
+
+Hint Extern 1 (environment ?E) =>
+  match goal with
+  | H : type_equal_core_validated E _ _ _ |- _ =>
+      apply (proj41 (type_equal_core_validated_inv H))
+  end : type_equal_core_validated.
+
+Hint Extern 1 (type ?T) =>
+  match goal with
+  | H : type_equal_core_validated _ T _ _ |- _ =>
+      apply (proj42 (type_equal_core_validated_inv H))
+  | H : type_equal_core_validated _ _ T _ |- _ =>
+      apply (proj43 (type_equal_core_validated_inv H))
+  end : type_equal_core_validated.
+
+Hint Extern 1 (kind ?K) =>
+  match goal with
+  | H : type_equal_core_validated _ _ _ K |- _ =>
+      apply (proj44 (type_equal_core_validated_inv H))
+  end : type_equal_core_validated.
+
+Hint Extern 1 (CSet.Nonempty ?cs) =>
+  match goal with
+  | H : type_equal_core_validated _ _ _ (knd_row cs) |- _ =>
+      let Hknd := fresh "Hknd" in
+      assert (kind (knd_row cs)) as Hknd
+        by apply (proj44 (type_equal_core_validated_inv H));
+      inversion Hknd; assumption
+  end : type_equal_core_validated.
+
+Lemma type_equal_cong_validated_inv : forall E T1 T2 K,
+    type_equal_cong_validated E T1 T2 K ->
+    environment E /\ type T1 /\ type T2 /\ kind K.
+Proof.
+  introv Hte.
+  destruct Hte; split; auto with csetdec.
+Qed.
+
+Hint Constructors type_equal_cong_validated : type_equal_cong_validated.
+
+Hint Extern 1 (environment ?E) =>
+  match goal with
+  | H : type_equal_cong_validated E _ _ _ |- _ =>
+      apply (proj41 (type_equal_cong_validated_inv H))
+  end : type_equal_cong_validated.
+
+Hint Extern 1 (type ?T) =>
+  match goal with
+  | H : type_equal_cong_validated _ T _ _ |- _ =>
+      apply (proj42 (type_equal_cong_validated_inv H))
+  | H : type_equal_cong_validated _ _ T _ |- _ =>
+      apply (proj43 (type_equal_cong_validated_inv H))
+  end : type_equal_cong_validated.
+
+Hint Extern 1 (kind ?K) =>
+  match goal with
+  | H : type_equal_cong_validated _ _ _ K |- _ =>
+      apply (proj44 (type_equal_cong_validated_inv H))
+  end : type_equal_cong_validated.
+
+Hint Extern 1 (CSet.Nonempty ?cs) =>
+  match goal with
+  | H : type_equal_cong_validated _ _ _ (knd_row cs) |- _ =>
+      let Hknd := fresh "Hknd" in
+      assert (kind (knd_row cs)) as Hknd
+        by apply (proj44 (type_equal_cong_validated_inv H));
+      inversion Hknd; assumption
+  end : type_equal_cong_validated.
+
+Lemma type_equal_symm_validated_inv : forall E T1 T2 K,
+    type_equal_symm_validated E T1 T2 K ->
+    environment E /\ type T1 /\ type T2 /\ kind K.
+Proof.
+  introv Hte.
+  destruct Hte; auto.
+Qed.
+
+Hint Constructors type_equal_symm_validated : type_equal_symm_validated.
+
+Hint Extern 1 (environment ?E) =>
+  match goal with
+  | H : type_equal_symm_validated E _ _ _ |- _ =>
+      apply (proj41 (type_equal_symm_validated_inv H))
+  end : type_equal_symm_validated.
+
+Hint Extern 1 (type ?T) =>
+  match goal with
+  | H : type_equal_symm_validated _ T _ _ |- _ =>
+      apply (proj42 (type_equal_symm_validated_inv H))
+  | H : type_equal_symm_validated _ _ T _ |- _ =>
+      apply (proj43 (type_equal_symm_validated_inv H))
+  end : type_equal_symm_validated.
+
+Hint Extern 1 (kind ?K) =>
+  match goal with
+  | H : type_equal_symm_validated _ _ _ K |- _ =>
+      apply (proj44 (type_equal_symm_validated_inv H))
+  end : type_equal_symm_validated.
+
+Hint Extern 1 (CSet.Nonempty ?cs) =>
+  match goal with
+  | H : type_equal_symm_validated _ _ _ (knd_row cs) |- _ =>
+      let Hknd := fresh "Hknd" in
+      assert (kind (knd_row cs)) as Hknd
+        by apply (proj44 (type_equal_symm_validated_inv H));
+      inversion Hknd; assumption
+  end : type_equal_symm_validated.
+
+Lemma type_equal_validated_inv : forall E T1 T2 K,
+    type_equal_validated E T1 T2 K ->
+    environment E /\ type T1 /\ type T2 /\ kind K.
+Proof.
+  introv Hk.
+  destruct Hk; auto.
+Qed.
+
+Hint Constructors type_equal_validated : type_equal_validated.
+
+Hint Extern 1 (environment ?E) =>
+  match goal with
+  | H : type_equal_validated E _ _ _ |- _ =>
+      apply (proj41 (type_equal_validated_inv H))
+  end : type_equal_validated.
+
+Hint Extern 1 (type ?T) =>
+  match goal with
+  | H : type_equal_validated _ T _ _ |- _ =>
+      apply (proj42 (type_equal_validated_inv H))
+  | H : type_equal_validated _ _ T _ |- _ =>
+      apply (proj43 (type_equal_validated_inv H))
+  end : type_equal_validated.
+
+Hint Extern 1 (kind ?K) =>
+  match goal with
+  | H : type_equal_validated _ _ _ K |- _ =>
+      apply (proj44 (type_equal_validated_inv H))
+  end : type_equal_validated.
+
+Hint Extern 1 (CSet.Nonempty ?cs) =>
+  match goal with
+  | H : type_equal_validated _ _ _ (knd_row cs) |- _ =>
+      let Hknd := fresh "Hknd" in
+      assert (kind (knd_row cs)) as Hknd
+        by apply (proj44 (type_equal_validated_inv H));
+      inversion Hknd; assumption
+  end : type_equal_validated.
+
+Lemma subtype_validated_inv : forall E T1 T2 cs,
+    subtype_validated E T1 T2 cs ->
+    environment E /\ type T1 /\ type T2 /\ CSet.Nonempty cs.
+Proof.
+  introv Hk.
+  destruct Hk; auto.
+Qed.
+
+Hint Constructors subtype_validated : subtype_validated.
+
+Hint Extern 1 (environment ?E) =>
+  match goal with
+  | H : subtype_validated E _ _ _ |- _ =>
+      apply (proj41 (subtype_validated_inv H))
+  end : subtype_validated.
+
+Hint Extern 1 (type ?T) =>
+  match goal with
+  | H : subtype_validated _ T _ _ |- _ =>
+      apply (proj42 (subtype_validated_inv H))
+  | H : subtype_validated _ _ T _ |- _ =>
+      apply (proj43 (subtype_validated_inv H))
+  end : subtype_validated.
+
+Hint Extern 1 (CSet.Nonempty ?cs) =>
+  match goal with
+  | H : subtype_validated _ _ _ cs |- _ =>
+      apply (proj44 (subtype_validated_inv H))
+  end : subtype_validated.
+
+Lemma validated_combined_kinding :
+  (forall E K, valid_kind E K -> valid_kind_validated E K)
+  /\ (forall E T K, kinding E T K -> kinding_validated E T K)
+  /\ (forall E M Xs,
+         valid_scheme_vars E M Xs -> valid_scheme_vars_validated E M Xs)
+  /\ (forall E M, valid_scheme E M -> valid_scheme_validated E M)
+  /\ (forall E, valid_env E -> valid_env_validated E)
+  /\ (forall E T1 T2 K,
+       type_equal_core E T1 T2 K -> type_equal_core_validated E T1 T2 K)
+  /\ (forall E T1 T2 K,
+       type_equal_cong E T1 T2 K -> type_equal_cong_validated E T1 T2 K)
+  /\ (forall E T1 T2 K,
+       type_equal_symm E T1 T2 K -> type_equal_symm_validated E T1 T2 K)
+  /\ (forall E T1 T2 K,
+       type_equal E T1 T2 K -> type_equal_validated E T1 T2 K)
+  /\ (forall E T1 T2 cs,
+       subtype E T1 T2 cs -> subtype_validated E T1 T2 cs).
+Proof.
+  apply combined_kinding_mutind; intros; subst;
+    econstr auto with valid_kind_validated kinding_validated
+           valid_scheme_vars_validated valid_scheme_validated
+           valid_env_validated type_equal_core_validated
+           type_equal_cong_validated type_equal_symm_validated
+           type_equal_validated subtype_validated.
+  - assert (environment E) by auto with valid_env_validated.
+    assert (kind K) by (eapply kind_from_env; eassumption).
+    auto with kinding_validated.
+  - assert (kind (knd_range T1 T2)) as Hknd
+      by auto with kinding_validated.
+    inversion Hknd; subst.
+    apply kinding_validated_variant with (T1 := T1) (T2 := T2);
+      auto with kinding_validated.
+  - apply valid_scheme_validated_c with (L := L); try assumption.
+    + pick_freshes_gen L (sch_arity M) Xs.
+      assert (valid_scheme_vars_validated E M Xs) by auto.
+      auto with valid_scheme_vars_validated.
+    + exists L. intros.
+      assert (valid_scheme_vars_validated E M Xs) by auto.
+      auto with valid_scheme_vars_validated.
+  - assert (kind (knd_range T2 T3)) as Hknd
+      by auto with type_equal_cong_validated.
+    inversion Hknd; subst.
+    auto with type_equal_cong_validated.
+  - assert (type (typ_meet T1 T2)) as Ht
+      by auto with type_equal_validated.
+    inversion Ht; subst.
+    auto with subtype_validated type_equal_validated.
+Qed.
+
+Lemma unvalidated_combined_kinding :
+  (forall E K, valid_kind_validated E K -> valid_kind E K)
+  /\ (forall E T K, kinding_validated E T K -> kinding E T K)
+  /\ (forall E M Xs,
+         valid_scheme_vars_validated E M Xs -> valid_scheme_vars E M Xs)
+  /\ (forall E M, valid_scheme_validated E M -> valid_scheme E M)
+  /\ (forall E, valid_env_validated E -> valid_env E)
+  /\ (forall E T1 T2 K,
+       type_equal_core_validated E T1 T2 K -> type_equal_core E T1 T2 K)
+  /\ (forall E T1 T2 K,
+       type_equal_cong_validated E T1 T2 K -> type_equal_cong E T1 T2 K)
+  /\ (forall E T1 T2 K,
+       type_equal_symm_validated E T1 T2 K -> type_equal_symm E T1 T2 K)
+  /\ (forall E T1 T2 K,
+       type_equal_validated E T1 T2 K -> type_equal E T1 T2 K)
+  /\ (forall E T1 T2 cs,
+       subtype_validated E T1 T2 cs -> subtype E T1 T2 cs).
+Proof.
+  apply combined_kinding_validated_mutind; intros; subst; econstr auto.
+Qed.
+
+Lemma validated_valid_kind : forall E K,
+    valid_kind E K -> valid_kind_validated E K.
+Proof.
+  pose validated_combined_kinding.
+  tauto.
+Qed.
+
+Lemma unvalidated_valid_kind : forall T1 T2,
+    valid_kind_validated T1 T2 -> valid_kind T1 T2.
+Proof.
+  pose unvalidated_combined_kinding.
+  tauto.
+Qed.
+
+Hint Resolve unvalidated_valid_kind.
+
+Hint Extern 1 (environment ?E) =>
+  match goal with
+  | H : valid_kind E _ |- _ =>
+      apply (proj1 (valid_kind_validated_inv
+                      (validated_valid_kind H)))
+  end : valid_kind_validated.
+
+Hint Extern 1 (kind ?K) =>
+  match goal with
+  | H : valid_kind _ K |- _ =>
+      apply (proj2 (valid_kind_validated_inv
+                      (validated_valid_kind H)))
+  end : valid_kind_validated.
+
+Lemma validated_kinding : forall E T K,
+    kinding E T K -> kinding_validated E T K.
+Proof.
+  pose validated_combined_kinding.
+  tauto.
+Qed.
+
+Lemma unvalidated_kinding : forall E T K,
+    kinding_validated E T K -> kinding E T K.
+Proof.
+  pose unvalidated_combined_kinding.
+  tauto.
+Qed.
+
+Hint Resolve unvalidated_kinding.
+
+Hint Extern 1 (environment ?E) =>
+  match goal with
+  | H : kinding E _ _ |- _ =>
+      apply (proj31 (kinding_validated_inv (validated_kinding H)))
+  end : kinding_validated.
+
+Hint Extern 1 (type ?T) =>
+  match goal with
+  | H : kinding _ T _ |- _ =>
+      apply (proj32 (kinding_validated_inv (validated_kinding H)))
+  end : kinding_validated.
+
+Hint Extern 1 (kind ?K) =>
+  match goal with
+  | H : kinding _ _ K |- _ =>
+      apply (proj33 (kinding_validated_inv (validated_kinding H)))
+  end : kinding_validated.
+
+Lemma validated_valid_scheme_vars : forall E M Xs,
+    valid_scheme_vars E M Xs -> valid_scheme_vars_validated E M Xs.
+Proof.
+  pose validated_combined_kinding.
+  tauto.
+Qed.
+
+Lemma unvalidated_valid_scheme_vars : forall E M Xs,
+    valid_scheme_vars_validated E M Xs -> valid_scheme_vars E M Xs.
+Proof.
+  pose unvalidated_combined_kinding.
+  tauto.
+Qed.
+
+Hint Resolve unvalidated_valid_scheme_vars.
+
+Hint Extern 1 (environment ?E) =>
+  match goal with
+  | H : valid_scheme_vars E _ _ |- _ =>
+      apply (proj1 (valid_scheme_vars_validated_inv
+                      (validated_valid_scheme_vars H)))
+  end : valid_scheme_vars_validated.
+
+Hint Extern 1 (scheme_vars ?M ?Xs) =>
+  match goal with
+  | H : valid_scheme_vars _ M Xs |- _ =>
+      apply (proj2 (valid_scheme_vars_validated_inv
+                      (validated_valid_scheme_vars H)))
+  end : valid_scheme_vars_validated.
+
+Lemma validated_valid_scheme : forall E M,
+    valid_scheme E M -> valid_scheme_validated E M.
+Proof.
+  pose validated_combined_kinding.
+  tauto.
+Qed.
+
+Lemma unvalidated_valid_scheme : forall E M,
+    valid_scheme_validated E M -> valid_scheme E M.
+Proof.
+  pose unvalidated_combined_kinding.
+  tauto.
+Qed.
+
+Hint Resolve unvalidated_valid_scheme.
+
+Hint Extern 1 (environment ?E) =>
+  match goal with
+  | H : valid_scheme E _ |- _ =>
+      apply (proj1 (valid_scheme_validated_inv
+                      (validated_valid_scheme H)))
+  end : valid_scheme_validated.
+
+Hint Extern 1 (scheme ?M) =>
+  match goal with
+  | H : valid_scheme _ M |- _ =>
+      apply (proj2 (valid_scheme_validated_inv
+                      (validated_valid_scheme H)))
+  end : valid_scheme_validated.
+
+Lemma validated_valid_env : forall E,
+    valid_env E -> valid_env_validated E.
+Proof.
+  pose validated_combined_kinding.
+  tauto.
+Qed.
+
+Lemma unvalidated_valid_env : forall E,
+    valid_env_validated E -> valid_env E.
+Proof.
+  pose unvalidated_combined_kinding.
+  tauto.
+Qed.
+
+Hint Resolve unvalidated_valid_env.
+
+Hint Extern 1 (environment ?E) =>
+  match goal with
+  | H : valid_env E |- _ =>
+      apply (valid_env_validated_inv
+               (validated_valid_env H))
+  end : valid_env_validated.
+
+Lemma validated_type_equal_core : forall E T1 T2 K,
+    type_equal_core E T1 T2 K -> type_equal_core_validated E T1 T2 K.
+Proof.
+  pose validated_combined_kinding.
+  tauto.
+Qed.
+
+Lemma unvalidated_type_equal_core : forall E T1 T2 K,
+    type_equal_core_validated E T1 T2 K -> type_equal_core E T1 T2 K.
+Proof.
+  pose unvalidated_combined_kinding.
+  tauto.
+Qed.
+
+Hint Resolve unvalidated_type_equal_core.
+
+Hint Extern 1 (environment ?E) =>
+  match goal with
+  | H : type_equal_core E _ _ _ |- _ =>
+      apply (proj41 (type_equal_core_validated_inv
+                       (validated_type_equal_core H)))
+  end : type_equal_core_validated.
+
+Hint Extern 1 (type ?T) =>
+  match goal with
+  | H : type_equal_core _ T _ _ |- _ =>
+      apply (proj42 (type_equal_core_validated_inv
+                       (validated_type_equal_core H)))
+  | H : type_equal_core _ _ T _ |- _ =>
+      apply (proj43 (type_equal_core_validated_inv
+                       (validated_type_equal_core H)))
+  end : type_equal_core_validated.
+
+Hint Extern 1 (kind ?K) =>
+  match goal with
+  | H : type_equal_core _ _ _ K |- _ =>
+      apply (proj44 (type_equal_core_validated_inv
+                       (validated_type_equal_core H)))
+  end : type_equal_core_validated.
+
+Lemma validated_type_equal_cong : forall E T1 T2 K,
+    type_equal_cong E T1 T2 K -> type_equal_cong_validated E T1 T2 K.
+Proof.
+  pose validated_combined_kinding.
+  tauto.
+Qed.
+
+Lemma unvalidated_type_equal_cong : forall E T1 T2 K,
+    type_equal_cong_validated E T1 T2 K -> type_equal_cong E T1 T2 K.
+Proof.
+  pose unvalidated_combined_kinding.
+  tauto.
+Qed.
+
+Hint Resolve unvalidated_type_equal_cong.
+
+Hint Extern 1 (environment ?E) =>
+  match goal with
+  | H : type_equal_cong E _ _ _ |- _ =>
+      apply (proj41 (type_equal_cong_validated_inv
+                       (validated_type_equal_cong H)))
+  end : type_equal_cong_validated.
+
+Hint Extern 1 (type ?T) =>
+  match goal with
+  | H : type_equal_cong _ T _ _ |- _ =>
+      apply (proj42 (type_equal_cong_validated_inv
+                       (validated_type_equal_cong H)))
+  | H : type_equal_cong _ _ T _ |- _ =>
+      apply (proj43 (type_equal_cong_validated_inv
+                       (validated_type_equal_cong H)))
+  end : type_equal_cong_validated.
+
+Hint Extern 1 (kind ?K) =>
+  match goal with
+  | H : type_equal_cong _ _ _ K |- _ =>
+      apply (proj44 (type_equal_cong_validated_inv
+                       (validated_type_equal_cong H)))
+  end : type_equal_cong_validated.
+
+Lemma validated_type_equal_symm : forall E T1 T2 K,
+    type_equal_symm E T1 T2 K -> type_equal_symm_validated E T1 T2 K.
+Proof.
+  pose validated_combined_kinding.
+  tauto.
+Qed.
+
+Lemma unvalidated_type_equal_symm : forall E T1 T2 K,
+    type_equal_symm_validated E T1 T2 K -> type_equal_symm E T1 T2 K.
+Proof.
+  pose unvalidated_combined_kinding.
+  tauto.
+Qed.
+
+Hint Resolve unvalidated_type_equal_symm.
+
+Hint Extern 1 (environment ?E) =>
+  match goal with
+  | H : type_equal_symm E _ _ _ |- _ =>
+      apply (proj41 (type_equal_symm_validated_inv
+                       (validated_type_equal_symm H)))
+  end : type_equal_symm_validated.
+
+Hint Extern 1 (type ?T) =>
+  match goal with
+  | H : type_equal_symm _ T _ _ |- _ =>
+      apply (proj42 (type_equal_symm_validated_inv
+                       (validated_type_equal_symm H)))
+  | H : type_equal_symm _ _ T _ |- _ =>
+      apply (proj43 (type_equal_symm_validated_inv
+                       (validated_type_equal_symm H)))
+  end : type_equal_symm_validated.
+
+Hint Extern 1 (kind ?K) =>
+  match goal with
+  | H : type_equal_symm _ _ _ K |- _ =>
+      apply (proj44 (type_equal_symm_validated_inv
+                       (validated_type_equal_symm H)))
+  end : type_equal_symm_validated.
+
+Lemma validated_type_equal : forall E T1 T2 K,
+    type_equal E T1 T2 K -> type_equal_validated E T1 T2 K.
+Proof.
+  pose validated_combined_kinding.
+  tauto.
+Qed.
+
+Lemma unvalidated_type_equal : forall E T1 T2 K,
+    type_equal_validated E T1 T2 K -> type_equal E T1 T2 K.
+Proof.
+  pose unvalidated_combined_kinding.
+  tauto.
+Qed.
+
+Hint Resolve unvalidated_type_equal.
+
+Hint Extern 1 (environment ?E) =>
+  match goal with
+  | H : type_equal E _ _ _ |- _ =>
+      apply (proj41 (type_equal_validated_inv
+                       (validated_type_equal H)))
+  end : type_equal_validated.
+
+Hint Extern 1 (type ?T) =>
+  match goal with
+  | H : type_equal _ T _ _ |- _ =>
+      apply (proj42 (type_equal_validated_inv
+                       (validated_type_equal H)))
+  | H : type_equal _ _ T _ |- _ =>
+      apply (proj43 (type_equal_validated_inv
+                       (validated_type_equal H)))
+  end : type_equal_validated.
+
+Hint Extern 1 (kind ?K) =>
+  match goal with
+  | H : type_equal _ _ _ K |- _ =>
+      apply (proj44 (type_equal_validated_inv
+                       (validated_type_equal H)))
+  end : type_equal_validated.
+
+Lemma validated_subtype : forall E T1 T2 K,
+    subtype E T1 T2 K -> subtype_validated E T1 T2 K.
+Proof.
+  pose validated_combined_kinding.
+  tauto.
+Qed.
+
+Lemma unvalidated_subtype : forall E T1 T2 K,
+    subtype_validated E T1 T2 K -> subtype E T1 T2 K.
+Proof.
+  pose unvalidated_combined_kinding.
+  tauto.
+Qed.
+
+Hint Resolve unvalidated_subtype.
+
+Hint Extern 1 (environment ?E) =>
+  match goal with
+  | H : subtype E _ _ _ |- _ =>
+      apply (proj41 (subtype_validated_inv
+                       (validated_subtype H)))
+  end : subtype_validated.
+
+Hint Extern 1 (type ?T) =>
+  match goal with
+  | H : subtype _ T _ _ |- _ =>
+      apply (proj42 (subtype_validated_inv
+                       (validated_subtype H)))
+  | H : subtype _ _ T _ |- _ =>
+      apply (proj43 (subtype_validated_inv
+                       (validated_subtype H)))
+  end : subtype_validated.
+
+Hint Extern 1 (CSet.Nonempty ?cs) =>
+  match goal with
+  | H : subtype _ _ _ cs |- _ =>
+      apply (proj44 (subtype_validated_inv
+                       (validated_subtype H)))
+  end : subtype_validated.
+
+Inductive valid_instance_validated : env -> list typ -> sch -> Prop :=
+  | valid_instance_validated_empty : forall E T,
+      kinding E T knd_type ->
+      environment E ->
+      type T ->
+      types (sch_arity (sch_empty T)) nil ->
+      valid_instance_validated E nil (sch_empty T)
+  | valid_instance_validated_bind : forall E K M T Ts,
+      kinding E T K ->
+      valid_instance_validated E Ts (M ^^ T) ->
+      environment E ->
+      type T ->
+      types (sch_arity M) Ts ->
+      scheme (M ^^ T) ->
+      kind K ->
+      types (sch_arity (sch_bind K M)) (T :: Ts) ->
+      valid_instance_validated E (T :: Ts) (sch_bind K M).
+
+Lemma valid_instance_validated_inv : forall E Ts M,
+    valid_instance_validated E Ts M ->
+    environment E /\ types (sch_arity M) Ts /\ scheme M.
+Proof.
+  introv Hi.
+  induction Hi; splits; auto.
+  assert (scheme (M ^^ T)) as Hs by assumption.
+  destruct Hs as [L Hs].
+  pick_fresh_gen (L \u sch_fv M) Y.
+  exists (L \u \{Y}).
+  introv Hl.
+  destruct Xs.
+  + contradict Hl.
+  + destruct Hl.
+    apply scheme_vars_bind; auto.
+    unfold sch_open_var.
+    rewrite sch_subst_intro with (X := Y); auto.
+    rewrite sch_subst_vars_type; autorewrite with rew_sch_arity; auto.
+    autorewrite with rew_sch_arity in *.
+    assert (scheme_vars (sch_open M T) Xs) as Hsv by auto.
+    rewrite sch_subst_intro with (X := Y) in Hsv; auto.
+    rewrite sch_subst_vars_type in Hsv;
+      autorewrite with rew_sch_arity; auto.
+Qed.
+
+Hint Constructors valid_instance_validated : valid_instance_validated.
+
+Hint Extern 1 (environment ?E) =>
+  match goal with
+  | H : valid_instance_validated E _ _ |- _ =>
+      apply (proj31 (valid_instance_validated_inv H))
+  end : valid_instance_validated.
+
+Hint Extern 1 (types (sch_arity ?M) ?Ts) =>
+  match goal with
+  | H : valid_instance_validated _ Ts M |- _ =>
+      apply (proj32 (valid_instance_validated_inv H))
+  end : valid_instance_validated.
+
+Hint Extern 1 (scheme ?M) =>
+  match goal with
+  | H : valid_instance_validated _ _ M |- _ =>
+      apply (proj33 (valid_instance_validated_inv H))
+  end : valid_instance_validated.
+
+Lemma validated_valid_instance : forall E Ts M,
+    valid_instance E Ts M -> valid_instance_validated E Ts M.
+Proof.
+  introv Hi.
+  induction Hi; auto with valid_instance_validated.
+  - auto with valid_instance_validated kinding_validated.
+  - assert (type T) by auto with kinding_validated.
+    assert (types (sch_arity (sch_open M T)) Ts) as Hts
+      by auto with valid_instance_validated.
+    destruct Hts as [Hl Hts].
+    apply valid_instance_validated_bind;
+      auto with valid_instance_validated kinding_validated.
+    + rewrite <- sch_open_arity with (U := T).
+      auto with valid_instance_validated.
+    + autorewrite with rew_sch_arity in Hl.
+      split; simpl; auto.
+Qed.
+
+Lemma unvalidated_valid_instance : forall E Ts M,
+    valid_instance_validated E Ts M -> valid_instance E Ts M.
+Proof.
+  introv Hi.
+  induction Hi; auto using valid_instance.
+Qed.
+
+Hint Resolve unvalidated_valid_instance.
+
+Hint Extern 1 (environment ?E) =>
+  match goal with
+  | H : valid_instance E _ _ |- _ =>
+      apply (proj31 (valid_instance_validated_inv
+                       (validated_valid_instance H)))
+  end : valid_instance_validated.
+
+Hint Extern 1 (types (sch_arity ?M) ?Ts) =>
+  match goal with
+  | H : valid_instance _ Ts M |- _ =>
+      apply (proj32 (valid_instance_validated_inv
+                       (validated_valid_instance H)))
+  end : valid_instance_validated.
+
+Hint Extern 1 (scheme ?M) =>
+  match goal with
+  | H : valid_instance_validated _ _ M |- _ =>
+      apply (proj33 (valid_instance_validated_inv
+                       (validated_valid_instance H)))
+  end : valid_instance_validated.
+
+Inductive typing_validated : env -> trm -> typ -> Prop :=
+  | typing_validated_var : forall E x M Us,
+      environment E ->
+      scheme M ->
+      types (sch_arity M) Us ->
+      type (instance M Us) ->
+      valid_env E -> 
+      binds x (bind_typ M) E -> 
+      valid_instance E Us M ->
+      typing_validated E (trm_fvar x) (instance M Us)
+  | typing_validated_abs : forall L E T1 T2 t1,
+      environment E ->
+      (forall x, x \notin L ->
+         environment (E & x ~ bind_typ (sch_empty T1))) ->
+      type T1 ->
+      type T2 ->
+      term_body t1 ->
+      (forall x, x \notin L -> 
+        typing_validated
+          (E & x ~ bind_typ (sch_empty T1)) (t1 ^ x) T2) -> 
+      typing_validated E (trm_abs t1) (typ_arrow T1 T2)
+  | typing_validated_app : forall E S T t1 t2, 
+      environment E ->
+      type S ->
+      type T ->
+      term t1 ->
+      term t2 ->
+      typing_validated E t1 (typ_arrow S T) ->
+      typing_validated E t2 S ->   
+      typing_validated E (trm_app t1 t2) T
+  | typing_validated_let : forall M L E T2 t1 t2,
+      environment E ->
+      (forall Xs, fresh L (sch_arity M) Xs ->
+         environment (E & Xs ~::* M)) ->
+      (forall x, x \notin L ->
+         environment (E & x ~ (bind_typ M))) -> 
+      type T2 ->
+      (forall Xs, fresh L (sch_arity M) Xs ->
+         type (instance_vars M Xs)) ->
+      scheme M ->
+      term t1 ->
+      term_body t2 ->
+      (forall Xs, fresh L (sch_arity M) Xs ->
+         typing_validated
+           (E & Xs ~::* M)
+           t1 (instance_vars M Xs)) ->
+      (forall x, x \notin L ->
+         typing_validated (E & x ~ (bind_typ M)) (t2 ^ x) T2) -> 
+      typing_validated E (trm_let t1 t2) T2
+  | typing_validated_constructor : forall c E T1 T2 T3 t,
+      environment E ->
+      type T1 ->
+      type T2 ->
+      type T3 ->
+      term t ->
+      kinding E T1 (knd_range (typ_top CSet.universe) T2) ->
+      subtype E
+        (typ_proj T2 (CSet.singleton c))
+        (typ_constructor c T3)
+        (CSet.singleton c) ->
+      typing_validated E t T3 ->
+      typing_validated E (trm_constructor c t) (typ_variant T1)
+  | typing_validated_match : forall c L E T1 T2 T3 T4 T5
+                          T6 T7 T8 t1 t2 t3,
+      environment E ->
+      (forall x, x \notin L ->
+         environment (E & x ~: (sch_empty (typ_variant T3)))) ->
+      (forall y, y \notin L -> 
+         environment (E & y ~: (sch_empty (typ_variant T5)))) ->
+      type T1 ->
+      type T2 ->
+      type T3 ->
+      type T4 ->
+      type T5 ->
+      type T6 ->
+      type T7 ->
+      type T8 ->
+      term t1 ->
+      term_body t2 ->
+      term_body t3 ->
+      kinding E T1 (knd_range T2 (typ_bot CSet.universe)) ->
+      kinding E T3 (knd_range (typ_top CSet.universe) T4) ->
+      kinding E T5 (knd_range (typ_top CSet.universe) T6) ->
+      subtype E
+        (typ_proj T2 (CSet.singleton c))
+        (typ_constructor c T7)
+        (CSet.singleton c) ->
+      subtype E
+        (typ_proj T2 (CSet.singleton c))
+        (typ_proj T4 (CSet.singleton c))
+        (CSet.singleton c) ->
+      subtype E
+        (typ_proj T2 (CSet.cosingleton c))
+        (typ_proj T6 (CSet.cosingleton c))
+        (CSet.cosingleton c) ->
+      typing_validated E t1 (typ_variant T1) ->
+      (forall x, x \notin L ->
+         typing_validated (E & x ~: (sch_empty (typ_variant T3)))
+                (t2 ^ x) T8) ->
+      (forall y, y \notin L -> 
+         typing_validated (E & y ~: (sch_empty (typ_variant T5)))
+                (t3 ^ y) T8) ->
+      typing_validated E (trm_match t1 c t2 t3) T8
+  | typing_validated_destruct : forall c L E T1 T2 T3 T4 t1 t2,
+      environment E ->
+      (forall x, x \notin L ->
+         environment (E & x ~: (sch_empty T3))) ->
+      type T1 ->
+      type T2 ->
+      type T3 ->
+      type T4 ->
+      term t1 ->
+      term_body t2 ->
+      kinding E T1 (knd_range T2 (typ_bot CSet.universe)) ->
+      subtype E
+        (typ_constructor c T3)
+        (typ_proj T2 (CSet.singleton c))
+        (CSet.singleton c) ->
+      typing_validated E t1 (typ_variant T1) ->
+      (forall x, x \notin L ->
+         typing_validated (E & x ~: (sch_empty T3))
+                (t2 ^ x) T4) ->
+      typing_validated E (trm_destruct t1 c t2) T4
+  | typing_validated_absurd : forall E T1 T2 t1,
+      environment E ->
+      type T1 ->
+      type T2 ->
+      term t1 ->
+      kinding E T1 (knd_range (typ_bot CSet.universe)
+                              (typ_bot CSet.universe)) ->
+      kinding E T2 knd_type ->
+      typing_validated E t1 (typ_variant T1) ->
+      typing_validated E (trm_absurd t1) T2.
+
+Lemma typing_validated_inv : forall E t T,
+    typing_validated E t T ->
+      environment E /\ term t /\ type T.
+Proof.
+  introv Ht.
+  induction Ht; auto.
+Qed.
+
+Hint Constructors typing_validated : typing_validated.
+
+Hint Extern 1 (environment ?E) =>
+  match goal with
+  | H : typing_validated E _ _ |- _ =>
+      apply (proj31 (typing_validated_inv H))
+  end : typing_validated.
+
+Hint Extern 1 (term ?t) =>
+  match goal with
+  | H : typing_validated _ t _ |- _ =>
+      apply (proj32 (typing_validated_inv H))
+  end : typing_validated.
+
+Hint Extern 1 (type ?T) =>
+  match goal with
+  | H : typing_validated _ _ T |- _ =>
+      apply (proj33 (typing_validated_inv H))
+  end : typing_validated.
+
+Lemma validated_typing : forall E t T,
+    typing E t T -> typing_validated E t T.
+Proof.
+  introv Ht.
+  induction Ht.
+  - assert (environment E)
+      by auto with valid_env_validated.
+    assert (scheme M)
+      by (eapply scheme_from_env; eassumption).
+    assert (types (sch_arity M) Us)
+      by auto with valid_instance_validated.   
+    assert (type (instance M Us))
+      by auto using scheme_instance_type.
+    auto with typing_validated.
+  - pick_fresh_gen L x.
+    assert (typing_validated (E & x ~: sch_empty T1) (t1 ^ x) T2)
+      by auto.
+    apply typing_validated_abs with (L := L); auto with typing_validated.
+    + eauto using environment_retract with typing_validated.
+    + intros y Hn.
+      assert (typing_validated (E & y ~: sch_empty T1) (t1 ^ y) T2)
+        by auto.
+      auto with typing_validated.
+    + rewrite scheme_empty_type.
+      eauto using scheme_from_env with typing_validated.
+    + exists L.
+      intros y Hny.
+      assert (typing_validated (E & y ~: sch_empty T1) (t1 ^ y) T2)
+        by auto.
+      auto with typing_validated.
+  - assert (type (typ_arrow S T)) as Hta
+      by auto with typing_validated.
+    inversion Hta; subst.
+    eauto with typing_validated.
+  - pick_freshes_gen L (sch_arity M) Xs.
+    assert (typing_validated (E & Xs ~::* M) t1 (instance_vars M Xs))
+      by auto.
+    pick_fresh_gen L x.
+    assert (typing_validated (E & x ~: M) (t2 ^ x) T2) by auto.
+    apply typing_validated_let with (M := M) (L := L);
+      auto with typing_validated.
+    + eauto using environment_retract with typing_validated.
+    + intros Ys Hf.
+      assert (typing_validated (E & Ys ~::* M) t1 (instance_vars M Ys))
+        by auto.
+      auto with typing_validated.
+    + intros y Hn.
+      assert (typing_validated (E & y ~: M) (t2 ^ y) T2)
+        by auto.
+      auto with typing_validated.
+    + intros Ys Hl.
+      assert (typing_validated (E & Ys ~::* M) t1 (instance_vars M Ys))
+        by auto.
+      auto with typing_validated.
+    + eauto using scheme_from_env with typing_validated.
+    + exists L.
+      intros y Hny.
+      assert (typing_validated (E & y ~: M) (t2 ^ y) T2)
+        by auto.
+      auto with typing_validated.
+  - assert (kind (knd_range (typ_top CSet.universe) T2)) as Hknd
+        by auto with kinding_validated.
+    inversion Hknd; subst.
+    apply typing_validated_constructor with (T2 := T2) (T3 := T3);
+      auto with typing_validated kinding_validated.
+  - assert
+      (kind (knd_range T2 (typ_bot CSet.universe))) as Hknd1
+        by auto with kinding_validated.
+    inversion Hknd1; subst.
+    assert
+      (kind (knd_range (typ_top CSet.universe) T4)) as Hknd2
+      by auto with kinding_validated.
+    inversion Hknd2; subst.
+    assert
+      (kind (knd_range (typ_top CSet.universe) T6)) as Hknd3
+      by auto with kinding_validated.
+    inversion Hknd3; subst.
+    pick_fresh_gen L x.
+    assert
+      (typing_validated (E & x ~: sch_empty (typ_variant T3)) 
+         (t2 ^ x) T8) by auto.
+    apply typing_validated_match
+      with (L := L) (T1 := T1) (T2 := T2) (T3 := T3)
+           (T4 := T4) (T5 := T5) (T6 := T6) (T7 := T7);
+      auto with typing_validated kinding_validated.
+    + intros y Hny.
+      assert
+        (typing_validated (E & y ~: sch_empty (typ_variant T3)) 
+                        (t2 ^ y) T8)
+        by auto.
+      auto with typing_validated.
+    + intros y Hny.
+      assert
+        (typing_validated (E & y ~: sch_empty (typ_variant T5)) 
+                        (t3 ^ y) T8)
+        by auto.
+      auto with typing_validated.
+    + assert (type (typ_constructor c T7)) as Hto
+          by auto with subtype_validated.
+      inversion Hto; subst.
+      assumption.
+    + exists L.
+      intros y Hny.
+      assert
+        (typing_validated (E & y ~: sch_empty (typ_variant T3)) 
+                        (t2 ^ y) T8)
+        by auto.
+      auto with typing_validated.
+    + exists L.
+      intros y Hny.
+      assert
+        (typing_validated (E & y ~: sch_empty (typ_variant T5)) 
+                        (t3 ^ y) T8)
+        by auto.
+      auto with typing_validated.
+  - apply typing_validated_destruct
+      with (L := L) (T1 := T1) (T2 := T2) (T3 := T3);
+      auto with typing_validated kinding_validated.
+    + intros y Hfy.
+      assert (typing_validated (E & y ~: sch_empty T3) (t2 ^ y) T4)
+        by auto.
+      auto with typing_validated.
+    + assert (type (typ_proj T2 (CSet.singleton c))) as Htp
+        by auto with subtype_validated.
+      inversion Htp; assumption.
+    + assert (type (typ_constructor c T3)) as Htc
+        by auto with subtype_validated.
+      inversion Htc; assumption.
+    + pick_fresh_gen L x.
+      assert (typing_validated (E & x ~: sch_empty T3) (t2 ^ x) T4)
+        by auto.
+      auto with typing_validated.
+    + exists L.
+      intros y Hny.
+      assert
+        (typing_validated (E & y ~: sch_empty T3) (t2 ^ y) T4)
+        by auto.
+      auto with typing_validated.
+  - apply typing_validated_absurd with (T1 := T1);
+      auto with typing_validated kinding_validated.
+Qed.
+
+Lemma unvalidated_typing : forall E t T,
+    typing_validated E t T -> typing E t T.
+Proof.
+  introv Ht.
+  induction Ht; eauto using typing.
+Qed.
+
+Hint Resolve unvalidated_typing.
+
+Hint Extern 1 (environment ?E) =>
+  match goal with
+  | H : typing E _ _ |- _ =>
+      apply (proj31 (typing_validated_inv (validated_typing H)))
+  end : typing_validated.
+
+Hint Extern 1 (term ?t) =>
+  match goal with
+  | H : typing _ t _ |- _ =>
+      apply (proj32 (typing_validated_inv (validated_typing H)))
+  end : typing_validated.
+
+Hint Extern 1 (type ?T) =>
+  match goal with
+  | H : typing _ _ T |- _ =>
+      apply (proj33 (typing_validated_inv (validated_typing H)))
+  end : typing_validated.
 
 (* *************************************************************** *)
-(** Preserved by type substitution *)
+(** * Convenient inversions of valid schemes *)
 
-Lemma kinding_env_typ_subst : forall E F X K T,
-  kinding_env (E & X ~:: K & F) -> 
-  kinding E T K -> 
-  kinding_env (E & (environment_subst X T F)).
+Lemma valid_scheme_bind_inv_sch : forall E K M X,
+    X # E ->
+    valid_scheme E (sch_bind K M) ->
+    valid_scheme (E & X ~:: K) (M ^ X).
 Proof.
-  introv He Hk.
-  induction F using env_ind.
-  - rewrite environment_subst_empty.
-    rewrite concat_empty_r.
-    eauto using kinding_env_shorten.
-  - rewrite environment_subst_push.
-    rewrite concat_assoc.
-    rewrite concat_assoc in He.
-    destruct v; simpl binding_subst.
-    + { destruct (kinding_env_kind_push_inv He).
-        apply kinding_env_kind; auto.
-        - lets Hee : (kinding_env_regular He).
-          apply kind_from_env with
-            (E := E & X ~:: K & F & x ~:: k)
-            (x := x); auto.
-        - rewrite dom_concat.
-          rewrite dom_environment_subst.
-          auto. }
-    + { destruct (kinding_env_typ_push_inv He) as [H1 [H2 H3]].
-        apply kinding_env_typ; auto.
-        - apply kinding_scheme_typ_subst with K; auto.
-        - rewrite dom_concat.
-          rewrite* dom_environment_subst. }
+  introv Hn Hs.
+  remember (sch_bind K M) as Mb.
+  destruct Hs; subst.
+  pick_fresh Y.
+  apply valid_scheme_c with (L := \{X} \u L \u \{Y}).
+  introv Hf.
+  fresh_length Hf as Hl.
+  autorewrite with rew_sch_arity in Hf.
+  assert (valid_scheme_vars E (sch_bind K M) (Y :: Xs)) as Hs by auto.
+  inversion Hs; subst.
+  assert (valid_env (E & Y ~:: K & X ~:: K)).
+  { apply valid_env_kind.
+
+  assert (Y \notin 
+  destruct Xs; simpl in Hl; inversion Hl.
+  inversion Hs; subst.
+
+  pick_fresh Y.
+  unfold sch_open_var.
+  rewrite sch_subst_intro with (X := Y); auto.
+  apply valid_scheme_typ_subst; auto.
+  exists (L \u \{Y}).
+  introv Hf.
+  specialize (Hs (Y :: Xs)).
+  simpl in Hs.
+  autorewrite with rew_sch_arity in Hf.
+  assert (scheme_vars (sch_bind K M) (Y :: Xs)) as Hsb by auto.
+  inversion Hsb; subst; auto.
+Qed.  
+
+Lemma valid_scheme_bind_inv_knd : forall E K M,
+    valid_scheme E (sch_bind K M) -> valid_kind E K.
+Proof.
+  introv Hs.
+  remember (sch_bind K M) as Mb.
+  destruct Hs; subst.
+  pick_freshes_gen L (sch_arity (sch_bind K M)) Xs.
+  fresh_length Fr as Hl.
+  assert (valid_scheme_vars E (sch_bind K M) Xs) as Hs by auto.
+  inversion Hs.
+  auto.
+Qed.  
+
+(* *************************************************************** *)
+(** * Constructor of valid "kinds" bindings  *)
+
+Lemma valid_env_kinds : forall E Xs M,
+    valid_env E ->
+    (fresh (dom E) (sch_arity M) Xs) ->
+    valid_scheme E M ->
+    valid_env (E & Xs ~::* M).
+Proof.
+  introv He Hf Hs.
+  fresh_length Hf as Hl.
+  rewrite <- (concat_empty_r E) in *.
+  generalize dependent (@empty bind).
+  generalize dependent M.
+  induction Xs; intros M Hl F He Hf Hs; simpl.
+  - autorewrite with rew_env_concat; auto.
+  - destruct M.
+    + autorewrite with rew_env_concat; auto.
+    + { destruct Hf.
+        rewrite concat_assoc.
+        rewrite <- (concat_assoc E).
+        apply IHXs.
+        - autorewrite with rew_sch_arity. auto.
+        - rewrite concat_assoc.
+          apply valid_env_kind; auto.
+          apply valid_scheme_bind_inv_knd with (M := M).
+          auto.
+        - autorewrite with rew_env_dom in *.
+          autorewrite with rew_sch_arity.
+          auto.
+        - }
 Qed.
 
-Hint Resolve kinding_env_typ_subst: typ_subst.
 
-Lemma kinding_closed : forall E T K X,
-    kinding E T K ->
-    X \in typ_fv T ->
-    X \in dom E.
+(* *************************************************************** *)
+(** A version of the symmetry lemma for type equality that does
+    not require separate evidence that the types involved are
+    well-kinded. *)
+
+Lemma type_equal_symmetric : forall E T1 T2 K,
+    type_equal E T1 T2 K ->
+    type_equal E T2 T1 K.
 Proof.
-  introv Hk Hfv.
-  induction Hk; simpl in Hfv; rew_in in Hfv; iauto.
-  subst.
-  eapply get_some_inv.
-  apply H0.
 Qed.
 
-Lemma kinding_scheme_closed : forall E M X,
-    kinding_scheme E M ->
-    X \in sch_fv M ->
-    X \in dom E.
+(* *************************************************************** *)
+(** Versions of the partial order lemmas for subtyping that do not
+    require separate evidence that the types involved are
+    well-kinded. *)
+
+Lemma subtype_reflexive : forall E T cs,
+    kinding E T (knd_row cs) ->
+    subtype E T T cs.
 Proof.
-  introv Hks Hfv.
-  unfold kinding_scheme, kinding_body in Hks.
-  unfold sch_fv in Hfv.
-  destruct Hks as [L Hk].
-  pick_freshes (sch_arity M) Xs.
-  destruct Hk with Xs as [_ Hkk]; auto.
-  eapply kinding_closed with (X := X) in Hkk; auto.
-  - rewrite dom_concat in Hkk.
-    rew_in in Hkk.
-    destruct* Hkk.
-    rewrite dom_map in H.
-    rewrite dom_singles in H.
-    + assert (fresh \{X} (sch_arity M) Xs) by auto.
-      eapply fresh_single_notin in H; auto.
-      tryfalse.
-    + apply fresh_length in Fr.
-      unfold sch_arity in Fr.
-      rewrite! liblist_length_eq_length.
-      auto.
-  - apply* typ_fv_open_vars.
+Qed.
+     
+Lemma subtype_transitive : forall E T1 T2 T3 cs,
+    subtype E T1 T2 cs ->
+    subtype E T2 T3 cs ->
+    subtype E T1 T3 cs.
+Proof.
 Qed.
 
-Lemma kinding_env_closed : forall E X,
-    kinding_env E ->
-    X \in env_fv E ->
-    X \in dom E.
+Lemma subtype_antisymmetric : forall E T1 T2 cs,
+    subtype E T1 T2 cs ->
+    subtype E T2 T1 cs ->
+    type_equal E T1 T2 (knd_row cs).
 Proof.
-  introv Hk Hfv.
-  induction Hk.
-  - rewrite env_fv_empty in Hfv.
-    rew_in in Hfv.
-    iauto.
-  - rewrite env_fv_push_inv in Hfv.
-    rewrite dom_push.
-    rew_in.
-    right.
-    rew_in in Hfv.
-    destruct* Hfv.
-  - rewrite env_fv_push_inv in Hfv.
-    rewrite dom_push.
-    rew_in.
-    right.
-    rew_in in Hfv.
-    destruct* Hfv.
-    simpl in H1.
-    apply kinding_scheme_closed with M; auto.
 Qed.
